moved most of resource defs and lemmas to a separate file

lawyer/nonblocking/examples/simple_queue.v
@@ -11,9 +11,6 @@ From iris.algebra Require Import auth gmap gset excl excl_auth csum mono_nat.
 From iris.base_logic.lib Require Import invariants.
 
 
-Close Scope Z.
-
-
 Class QueuePreG Σ := {
   q_pre_max :: MaxExactPreG Σ;
   q_pre_tok :: inG Σ (exclR unitO);
@@ -52,333 +49,312 @@ Class QueueG Σ := {
 }.
 
 
-Section SimpleQueue.
+Definition get_val: val := λ: "nd", ! ("nd" +ₗ #0).
+Definition get_next: val := λ: "nd", ! ("nd" +ₗ #1).
 
-  Definition get_val: val := λ: "nd", ! ("nd" +ₗ #0).
-  Definition get_next: val := λ: "nd", ! ("nd" +ₗ #1).
+Definition free_el: val. Admitted.
 
-  Definition free_el: val. Admitted.
+Definition get_to_free '(SQ _ _ BR FL _): val :=
+  λ: "ph",
+    if: ("ph" = !#BR)
+    then
+      let: "old_fl" := !#FL in
+      #FL <- "ph" ;;
+      "old_fl"
+    else "ph"
+.
 
-  Definition get_to_free '(SQ _ _ BR FL _): val :=
-    λ: "ph",
-      if: ("ph" = !#BR)
-      then
-        let: "old_fl" := !#FL in
-        #FL <- "ph" ;;
-        "old_fl"
-      else "ph"
-  .
+Definition dequeue '(SQ H T BR FL OHV as sq): val :=
+  λ: "q",
+    let: "c" := !#H in
+    if: ("c" = !#T)
+    then NONE
+    else
+      let: "v" := get_val "c" in
+      #OHV <- "v" ;;
+      #H <- (get_next "c") ;;
+      let: "to_free" := get_to_free sq "c" in
+      free_el "to_free" ;;
+      (SOME "v")
+.
 
-  Definition dequeue '(SQ H T BR FL OHV as sq): val :=
-    λ: "q",
-      let: "c" := !#H in
-      if: ("c" = !#T)
-        then NONE
-        else
-          let: "v" := get_val "c" in
-          #OHV <- "v" ;;
-          #H <- (get_next "c") ;;
-          let: "to_free" := get_to_free sq "c" in
-          free_el "to_free" ;;
-          (SOME "v")
-  .
 
-  Section QueueResources. 
+Section QueueResources. 
 
-    Context {Σ} {hG: heap1GS Σ} {iG: invGS_gen HasNoLc Σ}.
+  Context {Σ} {hG: heap1GS Σ} {iG: invGS_gen HasNoLc Σ}.
   
-    Context {QL: QueueG Σ}.
-
-    Definition hn_interp (hn: HistNode): iProp Σ :=
-      let '(l, (v, nxt)) := hn in
-      l ↦ v ∗ (l +ₗ 1) ↦ #nxt.
-
-    Definition dummy_node: Node := (#0, Loc 0).
-
-    Fixpoint is_LL_into (hq: HistQueue) (pt: loc) := 
-      match hq with 
-      | [] => True
-      | [ (_, (_, nxt)) ] => nxt = pt
-      (*   | (_, (_, nxt1)) :: ((l2, (_, _)) as hn2) :: hq' => nxt1 = l2 /\ is_LL (hn2 :: hq') *)
-      (** to avoid introducing Function *)
-      | (_, (_, nxt1)) :: hq' =>
-          match hq' with
-          | [] => True
-          | (l2, (_, _)) :: _ => nxt1 = l2 /\ is_LL_into hq' pt
-          end
-      end.
-
-    (** tail always points to a dummy node
-        which doesn NOT belong to the logical queue hq.
-        Upon enqueuing, this dummy note is updated and appended to hq.
-     *)
-    (* TODO: enforce it explicitly? *)
-    Definition queue_interp (hq: HistQueue) (h t br fl: nat): iProp Σ :=
-      ⌜ t = length hq ⌝ ∗ 
-      ([∗ list] nd ∈ drop h hq, hn_interp nd) ∗
-      ∃ (pt: loc), Tail q_sq ↦ #pt ∗ hn_interp (pt, dummy_node) ∗ ⌜ is_LL_into hq pt ⌝ ∗
-      let ph: loc := (from_option (fun hn => hn.1) pt (hq !! h)) in
-      Head q_sq ↦{1/2} #ph ∗
-      (∃ (nbr: HistNode), ⌜ hq !! br = Some nbr ⌝ ∗ BeingRead q_sq ↦#(nbr.1)) ∗
-      (∃ (nfl: HistNode), ⌜ hq !! fl = Some nfl ⌝ ∗ FreeLater q_sq ↦#(nfl.1) ∗ hn_interp nfl)
-    .
-
-    Lemma queue_interp_cur_empty (hq: HistQueue) (h br fl: nat):
-      queue_interp hq h h br fl -∗ ⌜ forall d, hq !! (h + d)%nat = None ⌝.
-    Proof using.
-      iIntros "(%&_)". subst. iPureIntro.
-      intros. apply lookup_ge_None_2. lia.
-    Qed.
-
-    (* TODO: try to get rid of if *)
-    Global Instance hni_tl hn: Timeless (hn_interp hn).
-    Proof using.
-      destruct hn as [? [??]]. apply _.
-    Defined. 
-
-    (* TODO: try to get rid of if *)
-    Global Instance qi_tl: forall hq h t br fl, Timeless (queue_interp hq h t br fl).
-    Proof using. 
-      intros. rewrite /queue_interp.
-      apply _. 
-    Defined.
-  
-    Definition dangle_auth (od: option nat): iProp Σ := own q_γ_dangle (●E od).
-    Definition dangle_frag (od: option nat): iProp Σ := own q_γ_dangle (◯E od).
-
-    Definition rop_auth (rop: option nat): iProp Σ := own q_γ_rop (●E rop).
-    Definition rop_frag (rop: option nat): iProp Σ := own q_γ_rop (◯E rop).
-      
-    Definition dangle_interp (od: option nat) (h: nat) (hq: HistQueue): iProp Σ :=
-      dangle_auth od ∗ (⌜ od = None ⌝ ∨ ⌜ od = Some (h - 1) ⌝ ∗ from_option hn_interp (⌜ False ⌝)%I (hq !! (h - 1)))
-    . 
-  
-    Definition auths (h t br fl: nat): iProp Σ :=
-      @me_auth _ q_me_h h ∗ @me_auth _ q_me_t t ∗ @me_auth _ q_me_br br ∗
-      @me_auth _ q_me_fl fl
-    .
-
-    Definition snapshot (h t br fl: nat): iProp Σ :=
-      @me_lb _ q_me_h h ∗ @me_lb _ q_me_t t ∗ @me_lb _ q_me_br br ∗
-      @me_lb _ q_me_fl fl
-    .
-
-    Lemma take_snapshot (h t br fl: nat): 
-      auths h t br fl -∗ snapshot h t br fl.
-    Proof using.
-      iIntros "(?&?&?&?)".
-      rewrite /snapshot. repeat iSplit; by iApply @me_auth_save.
-    Qed.
-
-    Lemma snapshot_lb (h t br fl: nat) (h' t' br' fl': nat):
-      snapshot h t br fl -∗ auths h' t' br' fl' -∗
-      ⌜ h <= h' /\ t <= t' /\ br <= br' /\ fl <= fl'⌝.
-    Proof using.
-      iIntros "#(X&?&?&?) (Y&?&?&?)".
-      repeat iSplit.
-      all: iApply (@me_auth_lb with "[-]"); eauto.
-    Qed.
-    
-    Definition cancel_witness (r: nat): iProp Σ :=
-      ∃ r', ⌜ r < r' ⌝ ∗ @me_lb _ q_me_h r'.
-
-    Definition rop_token: iProp Σ := own q_γ_tok_rop (Excl ()).
-
-    Definition safe_read (r: nat) (h br fl: nat) (od: option nat) rp: iProp Σ :=
-      ⌜ r = h ⌝ ∗ (⌜ rp = rs_init ⌝ ∨ ⌜ r = br ⌝ ∗ ⌜ rp = rs_proc (Some rsp_going) ⌝ ∗ rop_token) ∨
-      ⌜ r = h - 1 /\ r = br /\ is_Some od ⌝ ∗ ⌜ rp = rs_proc (Some rsp_protected) ⌝ ∨
-      ⌜ r = br /\ r = fl ⌝ ∗  ⌜ rp = rs_proc (Some rsp_protected) ⌝
-    .
-
-    Definition rop_interp (rop: option nat) (h br fl: nat) (od: option nat): iProp Σ :=
-      ∀ i, ⌜ rop = Some i  ⌝ -∗ ∃ r rp, ith_read i r 0 ∗ ith_rp i rp ∗
-                     (safe_read r h br fl od rp ∨ ⌜ rp = rs_canceled ⌝ ∗ cancel_witness r).
-  
-    Definition read_head_resources (t br: nat): iProp Σ :=
-      @me_exact _ q_me_t t ∗ @me_exact _ q_me_br br ∗ rop_frag None ∗ rop_token.
-
-    Definition dequeue_resources (h fl: nat) (ph: loc) (od: option nat): iProp Σ :=
-      @me_exact _ q_me_h h ∗ @me_exact _ q_me_fl fl ∗
-      Head q_sq ↦{1/2} #ph ∗ dangle_frag od. 
-  
-    Definition read_head_token: iProp Σ := own q_γ_tok_rh (Excl ()).
-    Definition dequeue_token: iProp Σ := own q_γ_tok_dq (Excl ()).
-
-    Definition hq_state_wf h t br fl: Prop :=
-      (* fl <= br /\ *) (* see runs.org for a counterexample *)
-      br <= h /\ fl < h /\ h <= t.
-      (* THIS IS FALSE: br can fall behind arbitrarily *)
-      (* (br = h \/ br = fl \/ od = Some (h - 1) /\ br = h - 1).  *)
-
-    Definition br_lb (b: nat) := @me_lb _ q_me_br b.
-
-    Definition read_hist_wf (hist: read_hist) (rop: option nat) (h: nat) :=
-      exists n, dom hist = set_seq 0 (S n) /\ (rop = None \/ rop = Some n) /\ 
-            (forall i j opi opj, i < j -> hist !! i = Some opi -> hist !! j = Some opj ->
-                             opi.1.2 <= opj.1.1) /\
-            (forall i opi, hist !! i = Some opi -> opi.1.1 <= h /\ opi.1.2 <= h).
-
-    Definition old_rps (hist: read_hist) (rop: option nat): iProp Σ :=
-      (* [∗ set] i ∈ (dom hist) ∖ (from_option (fun n => {[ n ]}) ∅ rop), *)
-      [∗ map] i ↦ '((r, b), rp) ∈ (from_option (fun n => delete n hist) hist rop),
-        (* (dom hist) ∖ (from_option (fun n => {[ n ]}) ∅ rop), *)
-              ∃ rp, ith_rp i rp ∗ ⌜ rs_fin rp ⌝ ∗
-                      (* (⌜ rp ≠ rs_canceled ⌝ -∗ br_lb b) *)
-                      br_lb r
-    
-    . 
-
-    (* TODO: upstream, find existing? *)
-    Global Instance Persistent_pure_helper P (R: iProp Σ) `{Decision P}:
-      (P -> Persistent R) -> Persistent (R ∗ ⌜ P ⌝).
-    Proof using.
-      intros PR. destruct (decide P).
-      - apply bi.sep_persistent; try by apply _. by apply PR.
-      - unshelve eapply bi.Persistent_proper. 1: exact (False)%I.
-        2: apply _. 
-        iSplit.
-        + by iIntros "(_&%)".
-        + by iIntros "?".
-    Qed.
-
-    Global Instance old_rps_pers: forall hist rop, Persistent (old_rps hist rop).
-    Proof using.
-      intros. rewrite /old_rps. apply big_sepM_persistent.
-      intros ? [[??] ?] ITH. simpl. 
-      apply bi.exist_persistent. intros rp.
-      rewrite bi.sep_assoc bi.sep_comm bi.sep_assoc. 
-      apply Persistent_pure_helper; [apply _| ]. 
-      intros. destruct H as [-> | [-> | ->]]; apply _.
-    Qed.
-    
-    Definition queue_inv_inner (hq: HistQueue) (h t br fl: nat)
-      (rop od: option nat) (hist: read_hist) (ohv: val): iProp Σ :=
-      hq_auth hq ∗ 
-      queue_interp hq h t br fl ∗ dangle_interp od h hq ∗ OldHeadVal q_sq↦ ohv ∗
-      ⌜ hq_state_wf h t br fl ⌝ ∗
-      auths h t br fl ∗
-      rop_interp rop h br fl od ∗
-      read_hist_auth hist ∗ ⌜ read_hist_wf hist rop h ⌝ ∗ old_rps hist rop ∗
-      (read_head_resources t br ∨ read_head_token) ∗ 
-      ((∃ ph, dequeue_resources h fl ph None) ∨ dequeue_token)
-    .
-  
-    Definition queue_ns := nroot .@ "queue".
-
-    Definition queue_at (q: val): iProp Σ :=
-      ⌜ q = (#(Head q_sq), (#(Tail q_sq), (#(BeingRead q_sq), (#(FreeLater q_sq), #(OldHeadVal q_sq)))))%V ⌝. 
-  
-    (* Definition queue_inv (q: loc): iProp Σ := *)
-    Definition queue_inv (q: val): iProp Σ :=
-      queue_at q ∗ inv queue_ns 
-        (∃ hq h t br fl rop od hist ohv, queue_inv_inner hq h t br fl rop od hist ohv)
-    .
-  
-    Lemma dequeue_token_excl:
-      dequeue_token -∗ dequeue_token -∗ False.
-    Proof using.
-      simpl. 
-      rewrite bi.wand_curry -own_op.
-      iIntros "X". by iDestruct (own_valid with "[$]") as %V.
-    Qed. 
-    
-    Lemma dequeue_resources_excl h1 fl1 ph1 od1 h2 fl2 ph2 od2:
-      dequeue_resources h1 fl1 ph1 od1 -∗ dequeue_resources h2 fl2 ph2 od2 -∗ False.
-    Proof using.
-      simpl. rewrite /dequeue_resources.
-      iIntros "(X&_) (Y&_)".
-      by iApply (me_exact_excl with "X [$]"). 
-    Qed.
-
-    Lemma dequeue_resources_auth_agree h' fl' ph od h t br fl:
-      dequeue_resources h' fl' ph od -∗ auths h t br fl -∗ ⌜ h' = h /\ fl' = fl ⌝.
-    Proof using.
-      simpl. iIntros "(H&FL&?&?) (H'&?&?&FL')".
-      iDestruct (me_auth_exact with "H' H") as %?. 
-      iDestruct (me_auth_exact with "FL' FL") as %?.
-      done. 
-    Qed. 
-    
-    Lemma dangle_auth_frag_agree od1 od2:
-      dangle_auth od1 -∗ dangle_frag od2 -∗ ⌜ od2 = od1 ⌝. 
-    Proof using.
-      simpl. rewrite /dangle_auth /dangle_frag.
-      rewrite bi.wand_curry -own_op.
-      iIntros "X". iDestruct (own_valid with "[$]") as %V.
-      iPureIntro. symmetry. by apply excl_auth_agree_L.
-    Qed.  
-    
-    Lemma dangle_update od1 od2 od':
-      dangle_auth od1 -∗ dangle_frag od2 ==∗ dangle_auth od' ∗ dangle_frag od'. 
-    Proof using.
-      simpl. rewrite /dangle_auth /dangle_frag.
-      rewrite bi.wand_curry -!own_op.
-      iApply own_update. apply excl_auth_update. 
-    Qed.  
-    
-    Lemma dequeue_resources_dangle_agree h fl ph od od' h' hq':
-      dequeue_resources h fl ph od -∗ dangle_interp od' h' hq' -∗ ⌜ od' = od ⌝.
-    Proof using.
-      simpl. iIntros "(?&?&?&FRAG) (AUTH&?)".
-      by iDestruct (dangle_auth_frag_agree with "[$] [$]") as %?. 
-    Qed.
-    
-    Lemma dequeue_res_head_agree h fl (ph ph': loc) od:
-      dequeue_resources h fl ph od -∗ Head q_sq ↦{1 / 2} #ph' -∗ ⌜ ph' = ph ⌝.
-    Proof using.
-      simpl. rewrite /dequeue_resources. iIntros "(_&_&H'&?) H".
-      iDestruct (pointsto_agree with "[$] [$]") as %?. set_solver.
-    Qed.
-    
-    Lemma cancel_rop h t br fl h'
-      (LT: h' < h):
-      auths h t br fl -∗ cancel_witness h'.
-    Proof using.
-      iIntros "(H&?&?&?)".
-      rewrite /cancel_witness.
-      iDestruct (me_auth_save with "H") as "LB".
-      iExists _. by iFrame.
-    Qed.
-    
-    Lemma old_rps_olds hist n:
-      old_rps hist (Some n) ⊣⊢ old_rps (delete n hist) None.
-    Proof using.
-      rewrite /old_rps. simpl. done. 
-    Qed.
-    
-    Lemma br_lb_bound b h t br fl:
-      br_lb b -∗ auths h t br fl -∗ ⌜ b <= br ⌝.
-    Proof using.
-      iIntros "LB (?&?&BR&?)".
-      iApply (me_auth_lb with "BR LB").
-    Qed.  
-
-    Lemma hn_interp_ptr_excl ptr nd1 nd2:
-      hn_interp (ptr, nd1) -∗ hn_interp (ptr, nd2) -∗ False.
-    Proof using.
-      simpl. destruct nd1, nd2. iIntros "[P1 ?] [P2 ?]".
-      iCombine "P1 P2" as "P". iDestruct (pointsto_valid with "P") as %V.
-      done.
-    Qed.
-
-  End QueueResources.
-
-
-  Context {DegO LvlO LIM_STEPS} {OP: OP_HL DegO LvlO LIM_STEPS}.
-  Context `{EM: ExecutionModel heap_lang M}.
-  Notation "'Degree'" := (om_hl_Degree). 
-  Notation "'Level'" := (om_hl_Level).  
-
-  Context {Σ} {OHE: OM_HL_Env OP EM Σ}.
-  (* Existing Instance OHE.  *)
   Context {QL: QueueG Σ}.
+  
+  Definition hn_interp (hn: HistNode): iProp Σ :=
+    let '(l, (v, nxt)) := hn in
+    l ↦ v ∗ (l +ₗ 1) ↦ #nxt.
 
-  Context (d: Degree).
+  Definition dummy_node: Node := (#0, Loc 0).
 
-  Definition get_loc_fuel := 5.
+  Fixpoint is_LL_into (hq: HistQueue) (pt: loc) := 
+    match hq with 
+    | [] => True
+    | [ (_, (_, nxt)) ] => nxt = pt
+    (*   | (_, (_, nxt1)) :: ((l2, (_, _)) as hn2) :: hq' => nxt1 = l2 /\ is_LL (hn2 :: hq') *)
+    (** to avoid introducing Function *)
+    | (_, (_, nxt1)) :: hq' =>
+        match hq' with
+        | [] => True
+        | (l2, (_, _)) :: _ => nxt1 = l2 /\ is_LL_into hq' pt
+        end
+    end.
 
-  Let hGS: heap1GS Σ := iem_phys _ EM.
-  Existing Instance hGS. 
+  (** tail always points to a dummy node
+      which doesn NOT belong to the logical queue hq.
+      Upon enqueuing, this dummy note is updated and appended to hq.
+   *)
+  (* TODO: enforce it explicitly? *)
+  Definition queue_interp (hq: HistQueue) (h t br fl: nat): iProp Σ :=
+    ⌜ t = length hq ⌝ ∗ 
+    ([∗ list] nd ∈ drop h hq, hn_interp nd) ∗
+    ∃ (pt: loc), Tail q_sq ↦ #pt ∗ hn_interp (pt, dummy_node) ∗ ⌜ is_LL_into hq pt ⌝ ∗
+    let ph: loc := (from_option (fun hn => hn.1) pt (hq !! h)) in
+    Head q_sq ↦{1/2} #ph ∗
+    (∃ (nbr: HistNode), ⌜ hq !! br = Some nbr ⌝ ∗ BeingRead q_sq ↦#(nbr.1)) ∗
+    (∃ (nfl: HistNode), ⌜ hq !! fl = Some nfl ⌝ ∗ FreeLater q_sq ↦#(nfl.1) ∗ hn_interp nfl)
+  .
+
+  Lemma queue_interp_cur_empty (hq: HistQueue) (h br fl: nat):
+    queue_interp hq h h br fl -∗ ⌜ forall d, hq !! (h + d)%nat = None ⌝.
+  Proof using.
+    iIntros "(%&_)". subst. iPureIntro.
+    intros. apply lookup_ge_None_2. lia.
+  Qed.
+  
+  (* TODO: try to get rid of if *)
+  Global Instance hni_tl hn: Timeless (hn_interp hn).
+  Proof using.
+    destruct hn as [? [??]]. apply _.
+  Defined. 
+  
+  (* TODO: try to get rid of if *)
+  Global Instance qi_tl: forall hq h t br fl, Timeless (queue_interp hq h t br fl).
+  Proof using. 
+    intros. rewrite /queue_interp.
+    apply _. 
+  Defined.
+  
+  Definition dangle_auth (od: option nat): iProp Σ := own q_γ_dangle (●E od).
+  Definition dangle_frag (od: option nat): iProp Σ := own q_γ_dangle (◯E od).
+  
+  Definition rop_auth (rop: option nat): iProp Σ := own q_γ_rop (●E rop).
+  Definition rop_frag (rop: option nat): iProp Σ := own q_γ_rop (◯E rop).
+  
+  Definition dangle_interp (od: option nat) (h: nat) (hq: HistQueue): iProp Σ :=
+    dangle_auth od ∗ (⌜ od = None ⌝ ∨ ⌜ od = Some (h - 1) ⌝ ∗ from_option hn_interp (⌜ False ⌝)%I (hq !! (h - 1)))
+  . 
+  
+  Definition auths (h t br fl: nat): iProp Σ :=
+    @me_auth _ q_me_h h ∗ @me_auth _ q_me_t t ∗ @me_auth _ q_me_br br ∗
+    @me_auth _ q_me_fl fl
+  .
+
+  Definition snapshot (h t br fl: nat): iProp Σ :=
+    @me_lb _ q_me_h h ∗ @me_lb _ q_me_t t ∗ @me_lb _ q_me_br br ∗
+    @me_lb _ q_me_fl fl
+  .
+
+  Lemma take_snapshot (h t br fl: nat): 
+    auths h t br fl -∗ snapshot h t br fl.
+  Proof using.
+    iIntros "(?&?&?&?)".
+    rewrite /snapshot. repeat iSplit; by iApply @me_auth_save.
+  Qed.
+
+  Lemma snapshot_lb (h t br fl: nat) (h' t' br' fl': nat):
+    snapshot h t br fl -∗ auths h' t' br' fl' -∗
+    ⌜ h <= h' /\ t <= t' /\ br <= br' /\ fl <= fl'⌝.
+  Proof using.
+    iIntros "#(X&?&?&?) (Y&?&?&?)".
+    repeat iSplit.
+    all: iApply (@me_auth_lb with "[-]"); eauto.
+  Qed.
+    
+  Definition cancel_witness (r: nat): iProp Σ :=
+    ∃ r', ⌜ r < r' ⌝ ∗ @me_lb _ q_me_h r'.
+
+  Definition rop_token: iProp Σ := own q_γ_tok_rop (Excl ()).
+
+  Definition safe_read (r: nat) (h br fl: nat) (od: option nat) rp: iProp Σ :=
+    ⌜ r = h ⌝ ∗ (⌜ rp = rs_init ⌝ ∨ ⌜ r = br ⌝ ∗ ⌜ rp = rs_proc (Some rsp_going) ⌝ ∗ rop_token) ∨
+    ⌜ r = h - 1 /\ r = br /\ is_Some od ⌝ ∗ ⌜ rp = rs_proc (Some rsp_protected) ⌝ ∨
+    ⌜ r = br /\ r = fl ⌝ ∗  ⌜ rp = rs_proc (Some rsp_protected) ⌝
+  .
+
+  Definition rop_interp (rop: option nat) (h br fl: nat) (od: option nat): iProp Σ :=
+    ∀ i, ⌜ rop = Some i  ⌝ -∗ ∃ r rp, ith_read i r 0 ∗ ith_rp i rp ∗
+        (safe_read r h br fl od rp ∨ ⌜ rp = rs_canceled ⌝ ∗ cancel_witness r).
+  
+  Definition read_head_resources (t br: nat): iProp Σ :=
+    @me_exact _ q_me_t t ∗ @me_exact _ q_me_br br ∗ rop_frag None ∗ rop_token.
+
+  Definition dequeue_resources (h fl: nat) (ph: loc) (od: option nat): iProp Σ :=
+    @me_exact _ q_me_h h ∗ @me_exact _ q_me_fl fl ∗
+    Head q_sq ↦{1/2} #ph ∗ dangle_frag od. 
+  
+  Definition read_head_token: iProp Σ := own q_γ_tok_rh (Excl ()).
+  Definition dequeue_token: iProp Σ := own q_γ_tok_dq (Excl ()).
+
+  Definition hq_state_wf h t br fl: Prop :=
+    (* fl <= br /\ *) (* see runs.org for a counterexample *)
+    br <= h /\ fl < h /\ h <= t.
+    (* THIS IS FALSE: br can fall behind arbitrarily *)
+    (* (br = h \/ br = fl \/ od = Some (h - 1) /\ br = h - 1).  *)
+
+  Definition br_lb (b: nat) := @me_lb _ q_me_br b.
+
+  Definition read_hist_wf (hist: read_hist) (rop: option nat) (h: nat) :=
+    exists n, dom hist = set_seq 0 (S n) /\ (rop = None \/ rop = Some n) /\ 
+           (forall i j opi opj, i < j -> hist !! i = Some opi -> hist !! j = Some opj ->
+                           opi.1.2 <= opj.1.1) /\
+           (forall i opi, hist !! i = Some opi -> opi.1.1 <= h /\ opi.1.2 <= h).
+
+  Definition old_rps (hist: read_hist) (rop: option nat): iProp Σ :=
+    (* [∗ set] i ∈ (dom hist) ∖ (from_option (fun n => {[ n ]}) ∅ rop), *)
+    [∗ map] i ↦ '((r, b), rp) ∈ (from_option (fun n => delete n hist) hist rop),
+      (* (dom hist) ∖ (from_option (fun n => {[ n ]}) ∅ rop), *)
+      ∃ rp, ith_rp i rp ∗ ⌜ rs_fin rp ⌝ ∗
+              (* (⌜ rp ≠ rs_canceled ⌝ -∗ br_lb b) *)
+              br_lb r
+  . 
+
+  (* TODO: upstream, find existing? *)
+  Global Instance Persistent_pure_helper P (R: iProp Σ) `{Decision P}:
+    (P -> Persistent R) -> Persistent (R ∗ ⌜ P ⌝).
+  Proof using.
+    intros PR. destruct (decide P).
+    - apply bi.sep_persistent; try by apply _. by apply PR.
+    - unshelve eapply bi.Persistent_proper. 1: exact (False)%I.
+      2: apply _. 
+      iSplit.
+      + by iIntros "(_&%)".
+      + by iIntros "?".
+  Qed.
+
+  Global Instance old_rps_pers: forall hist rop, Persistent (old_rps hist rop).
+  Proof using.
+    intros. rewrite /old_rps. apply big_sepM_persistent.
+    intros ? [[??] ?] ITH. simpl. 
+    apply bi.exist_persistent. intros rp.
+    rewrite bi.sep_assoc bi.sep_comm bi.sep_assoc. 
+    apply Persistent_pure_helper; [apply _| ]. 
+    intros. destruct H as [-> | [-> | ->]]; apply _.
+  Qed.
+    
+  Definition queue_inv_inner (hq: HistQueue) (h t br fl: nat)
+    (rop od: option nat) (hist: read_hist) (ohv: val): iProp Σ :=
+    hq_auth hq ∗ 
+    queue_interp hq h t br fl ∗ dangle_interp od h hq ∗ OldHeadVal q_sq↦ ohv ∗
+    ⌜ hq_state_wf h t br fl ⌝ ∗
+    auths h t br fl ∗
+    rop_interp rop h br fl od ∗
+    read_hist_auth hist ∗ ⌜ read_hist_wf hist rop h ⌝ ∗ old_rps hist rop ∗
+    (read_head_resources t br ∨ read_head_token) ∗ 
+    ((∃ ph, dequeue_resources h fl ph None) ∨ dequeue_token)
+  .
+  
+  Definition queue_ns := nroot .@ "queue".
+
+  Definition queue_at (q: val): iProp Σ :=
+    ⌜ q = (#(Head q_sq), (#(Tail q_sq), (#(BeingRead q_sq), (#(FreeLater q_sq), #(OldHeadVal q_sq)))))%V ⌝. 
+  
+  (* Definition queue_inv (q: loc): iProp Σ := *)
+  Definition queue_inv (q: val): iProp Σ :=
+    queue_at q ∗ inv queue_ns 
+      (∃ hq h t br fl rop od hist ohv, queue_inv_inner hq h t br fl rop od hist ohv)
+  .
+  
+  Lemma dequeue_token_excl:
+    dequeue_token -∗ dequeue_token -∗ False.
+  Proof using.
+    simpl. 
+    rewrite bi.wand_curry -own_op.
+    iIntros "X". by iDestruct (own_valid with "[$]") as %V.
+  Qed. 
+    
+  Lemma dequeue_resources_excl h1 fl1 ph1 od1 h2 fl2 ph2 od2:
+    dequeue_resources h1 fl1 ph1 od1 -∗ dequeue_resources h2 fl2 ph2 od2 -∗ False.
+  Proof using.
+    simpl. rewrite /dequeue_resources.
+    iIntros "(X&_) (Y&_)".
+    by iApply (me_exact_excl with "X [$]"). 
+  Qed.
+
+  Lemma dequeue_resources_auth_agree h' fl' ph od h t br fl:
+    dequeue_resources h' fl' ph od -∗ auths h t br fl -∗ ⌜ h' = h /\ fl' = fl ⌝.
+  Proof using.
+    simpl. iIntros "(H&FL&?&?) (H'&?&?&FL')".
+    iDestruct (me_auth_exact with "H' H") as %?. 
+    iDestruct (me_auth_exact with "FL' FL") as %?.
+    done. 
+  Qed. 
+    
+  Lemma dangle_auth_frag_agree od1 od2:
+    dangle_auth od1 -∗ dangle_frag od2 -∗ ⌜ od2 = od1 ⌝. 
+  Proof using.
+    simpl. rewrite /dangle_auth /dangle_frag.
+    rewrite bi.wand_curry -own_op.
+    iIntros "X". iDestruct (own_valid with "[$]") as %V.
+    iPureIntro. symmetry. by apply excl_auth_agree_L.
+  Qed.  
+    
+  Lemma dangle_update od1 od2 od':
+    dangle_auth od1 -∗ dangle_frag od2 ==∗ dangle_auth od' ∗ dangle_frag od'. 
+  Proof using.
+    simpl. rewrite /dangle_auth /dangle_frag.
+    rewrite bi.wand_curry -!own_op.
+    iApply own_update. apply excl_auth_update. 
+  Qed.  
+    
+  Lemma dequeue_resources_dangle_agree h fl ph od od' h' hq':
+    dequeue_resources h fl ph od -∗ dangle_interp od' h' hq' -∗ ⌜ od' = od ⌝.
+  Proof using.
+    simpl. iIntros "(?&?&?&FRAG) (AUTH&?)".
+    by iDestruct (dangle_auth_frag_agree with "[$] [$]") as %?. 
+  Qed.
+    
+  Lemma dequeue_res_head_agree h fl (ph ph': loc) od:
+    dequeue_resources h fl ph od -∗ Head q_sq ↦{1 / 2} #ph' -∗ ⌜ ph' = ph ⌝.
+  Proof using.
+    simpl. rewrite /dequeue_resources. iIntros "(_&_&H'&?) H".
+    iDestruct (pointsto_agree with "[$] [$]") as %?. set_solver.
+  Qed.
+    
+  Lemma cancel_rop h t br fl h'
+    (LT: h' < h):
+    auths h t br fl -∗ cancel_witness h'.
+  Proof using.
+    iIntros "(H&?&?&?)".
+    rewrite /cancel_witness.
+    iDestruct (me_auth_save with "H") as "LB".
+    iExists _. by iFrame.
+  Qed.
+    
+  Lemma old_rps_olds hist n:
+    old_rps hist (Some n) ⊣⊢ old_rps (delete n hist) None.
+  Proof using.
+    rewrite /old_rps. simpl. done. 
+  Qed.
+    
+  Lemma br_lb_bound b h t br fl:
+    br_lb b -∗ auths h t br fl -∗ ⌜ b <= br ⌝.
+  Proof using.
+    iIntros "LB (?&?&BR&?)".
+    iApply (me_auth_lb with "BR LB").
+  Qed.  
+
+  Lemma hn_interp_ptr_excl ptr nd1 nd2:
+    hn_interp (ptr, nd1) -∗ hn_interp (ptr, nd2) -∗ False.
+  Proof using.
+    simpl. destruct nd1, nd2. iIntros "[P1 ?] [P2 ?]".
+    iCombine "P1 P2" as "P". iDestruct (pointsto_valid with "P") as %V.
+    done.
+  Qed.
 
   Lemma access_queue_ends hq h t br fl:
     hq_auth hq -∗ queue_interp hq h t br fl -∗
@@ -425,542 +401,6 @@ Section SimpleQueue.
     iFrame. iIntros. iSplit; [done| ]. by iApply "CLOS".     
   Qed. 
 
-  Lemma get_head_val_spec Q τ π q h nd fl ph od:
-    {{{ queue_inv Q ∗ ith_node h (ph, nd) ∗ dequeue_resources h fl ph od ∗
-        th_phase_frag τ π q ∗ cp_mul π d get_loc_fuel }}}
-      get_val #ph @τ
-    {{{ RET (nd.1); th_phase_frag τ π q ∗ dequeue_resources h fl ph od }}}.
-  Proof using.
-    simpl. iIntros (Φ) "([#QAT #INV] & #HEADhn & DR & PH & CPS) POST".
-    rewrite /get_val.
-    destruct nd as [v nxt]. simpl.
-    pure_steps.
-    wp_bind (_ +ₗ _)%E.
-    iApply sswp_MU_wp; [done| ].
-    iApply sswp_pure_step; [done| ].
-    MU_by_burn_cp. rewrite loc_add_0. iApply wp_value.
-    iInv "INV" as "(%hq & %h_ & %t & %br & %fl_ & %rop & %od_ & %hist & %ohv & inv)" "CLOS".
-    iEval (rewrite /queue_inv_inner) in "inv".
-    iDestruct "inv" as "(>HQ & >QI & DANGLE & OHV & >%ORDER & >AUTHS & >ROP & RHIST & >%RH_WF & RH & DQ)".
-    iDestruct (dequeue_resources_auth_agree with "[$] [$]") as %[<- <-].
-    iDestruct "DR" as "[HEAD FL]".
-    iDestruct (hq_auth_lookup with "[$] [$]") as %HTH.
-    iAssert (⌜ t ≠ h ⌝)%I as %NEMPTY.
-    { iIntros (->). iDestruct (queue_interp_cur_empty with "[$]") as %NO.
-      specialize (NO 0). rewrite Nat.add_0_r in NO. congruence. } 
-    iDestruct (access_queue with "[$] [$] [$]") as "[HNI CLOS']".
-    { red in ORDER. lia. }
-    rewrite {1}/hn_interp. iDestruct "HNI" as "[VAL NXT]".
-    iApply sswp_MU_wp; [done| ].
-    iApply (wp_load with "VAL"). iIntros "!> VAL". 
-    MU_by_burn_cp. iApply wp_value.
-    iDestruct ("CLOS'" with "[$VAL $NXT]") as "[??]".
-    iMod ("CLOS" with "[-POST PH HEAD FL]") as "_".
-    { by iFrame. }
-    iModIntro. iApply "POST". iFrame.
-  Qed.
-
-  (* TODO: unify with the proof above *)
-  Lemma get_head_next_spec Q τ π q h nd fl ph od:
-    {{{ queue_inv Q ∗ ith_node h (ph, nd) ∗ dequeue_resources h fl ph od ∗
-        th_phase_frag τ π q ∗ cp_mul π d get_loc_fuel }}}
-      get_next #ph @τ
-    {{{ RET #(nd.2); th_phase_frag τ π q ∗ dequeue_resources h fl ph od }}}.
-  Proof using.
-    simpl. iIntros (Φ) "([#QAT #INV] & #HEADhn & DR & PH & CPS) POST".
-    rewrite /get_next.
-    destruct nd as [v nxt]. simpl.
-    pure_steps.
-    wp_bind (_ +ₗ _)%E.
-    iApply sswp_MU_wp; [done| ].
-    iApply sswp_pure_step; [done| ].
-    MU_by_burn_cp. iApply wp_value.
-    iInv "INV" as "(%hq & %h_ & %t & %br & %fl_ & %rop & %od' & %hist & %ohv & inv)" "CLOS".
-    iEval (rewrite /queue_inv_inner) in "inv".
-    iDestruct "inv" as "(>HQ & >QI & DANGLE & OHV & >%ORDER & >AUTHS & >ROP & RHIST & >%RH_WF & RH & DQ)".
-    iDestruct (dequeue_resources_auth_agree with "[$] [$]") as %[<- <-].
-    iDestruct "DR" as "[HEAD FL]".
-    iDestruct (hq_auth_lookup with "[$] [$]") as %HTH.
-    iAssert (⌜ t ≠ h ⌝)%I as %NEMPTY.
-    { iIntros (->). iDestruct (queue_interp_cur_empty with "[$]") as %NO.
-      specialize (NO 0). rewrite Nat.add_0_r in NO. congruence. } 
-    iDestruct (access_queue with "[$] [$] [$]") as "[HNI CLOS']".
-    { red in ORDER. lia. }
-    rewrite {1}/hn_interp. iDestruct "HNI" as "[VAL NXT]".
-    iApply sswp_MU_wp; [done| ].
-    iApply (wp_load with "NXT"). iIntros "!> NXT". 
-    MU_by_burn_cp. iApply wp_value.
-    iDestruct ("CLOS'" with "[$VAL $NXT]") as "[??]".
-    iMod ("CLOS" with "[-POST PH HEAD FL]") as "_".
-    { by iFrame. }
-    iModIntro. iApply "POST". iFrame.
-  Qed.
-
-  Lemma update_ohv_spec τ π q (v: val) l:
-    {{{ queue_inv l ∗ th_phase_frag τ π q ∗ cp_mul π d get_loc_fuel }}}
-      #(OldHeadVal q_sq) <- v @τ
-    {{{ RET #(); th_phase_frag τ π q }}}.
-  Proof using.
-    iIntros (Φ) "([#QAT #INV] & PH & CPS) POST".
-    iInv "INV" as "(%hq & %h & %t & %br & %fl & %rop & %od & %hist & %ohv & inv)" "CLOS".
-    iEval (rewrite /queue_inv_inner) in "inv".
-    iDestruct "inv" as "(>HQ & >QI & DANGLE & OHV & >%ORDER & >AUTHS & >ROP & RHIST & >%RH_WF & RH & DQ)".
-
-    iApply sswp_MU_wp; [done| ].
-    iApply (wp_store with "[$]"). iIntros "!> ?".
-    MU_by_burn_cp. iApply wp_value.
-    iMod ("CLOS" with "[-POST PH]") as "_". 
-    { by iFrame. }
-    by iApply "POST".
-  Qed.
-
-  Lemma is_LL_into_drop hq pt k
-    (LL: is_LL_into hq pt):
-    is_LL_into (drop k hq) pt.
-  Proof using.
-    revert k. induction hq.
-    { intros. by rewrite drop_nil. }
-    intros. destruct k.
-    { by rewrite drop_0. }
-    simpl. apply IHhq.
-    simpl in LL. destruct a as [? [? ?]].
-    destruct hq; try done.
-    destruct h as [? [? ?]]. tauto.
-  Qed.
-
-  Lemma dom_max_set_fold n:
-    set_fold max 0 (set_seq 0 (S n): gset nat) = n.
-  Proof using.
-    clear. induction n.
-    { done. }
-    rewrite set_seq_S_end_union_L.
-    rewrite union_comm_L. 
-    erewrite set_fold_union.
-    2-4: red; lia.
-    simpl. rewrite IHn.
-    rewrite set_fold_singleton. lia.
-  Qed.
-
-  Definition upd_rp rp :=
-    match rp with
-    | rs_init => rs_canceled
-    | rs_proc (Some rsp_going) => rs_proc (Some rsp_protected)
-    | _ => rp
-    end. 
-
-  Lemma upd_rp_rs_step p: rs_step p (upd_rp p).
-  Proof using.
-    destruct p; simpl; try constructor.
-    destruct orsp; simpl; try constructor.
-    destruct r; repeat constructor.
-  Qed.
-
-  Lemma read_hist_wf_bump (hist: read_hist) rop h rp
-    (RH_WF: read_hist_wf hist rop h)
-    (n := set_fold max 0 (dom hist)):
-  read_hist_auth hist
-    -∗ ith_rp n rp
-    ==∗
-  ∃ r rp',
-         let hist' := <[ n := ((r, h + 1), rp') ]> hist in
-         read_hist_auth hist' ∗ ith_read n r (h + 1) ∗ ⌜ read_hist_wf hist' rop (h + 1) ⌝ ∗
-         ith_rp n (upd_rp rp) ∗
-         ⌜ r <= h ⌝.
-  Proof using.
-    rewrite /read_hist_wf. iIntros "AUTH RP".
-    destruct RH_WF as (n_ & DOM & ROP & SEQ & BB).
-
-    assert (n_ = n) as ->.
-    { subst n. rewrite DOM. by rewrite dom_max_set_fold. }
-
-    destruct (hist !! n) as [[[r b0] p]| ] eqn:NTH.
-    2: { apply not_elem_of_dom in NTH. rewrite DOM in NTH.
-         rewrite elem_of_set_seq in NTH. lia. }
-    iDestruct (ith_rp_hist_compat with "[$] [$]") as %(? & ? & EQ').
-    rewrite NTH in H. inversion H. subst x. simpl in EQ'. clear H.
-    rename rp into p_. 
-    
-    iMod (read_hist_update' _ _ _ _ _ (h + 1) with "AUTH RP") as "(AUTH & #ITH & RP)".
-    { apply upd_rp_rs_step. }
-    { apply NTH. }
-
-    rewrite Nat.max_r.
-    2: { apply BB in NTH. simpl in NTH. lia. }
-    iModIntro. do 2 iExists _. iFrame "AUTH ITH RP".
-    iPureIntro. split.
-    2: { eapply BB in NTH; eauto. by apply NTH. }
-
-    exists n. split; [| split; [| split]]. 
-    - rewrite dom_insert_L. apply mk_is_Some, elem_of_dom in NTH. set_solver.
-    - done.
-    - intros ?????. rewrite !lookup_insert_Some.
-      intros [(? & ?) | (? & ITH) ] [(? & ?) | (? & JTH) ]; subst; simpl in *; try lia.
-      + apply mk_is_Some, elem_of_dom in JTH.
-        rewrite DOM elem_of_union elem_of_set_seq elem_of_singleton in JTH. lia.
-      + eapply SEQ in H; eauto. done.
-      + eapply SEQ; eauto.
-    - intros ??. rewrite lookup_insert_Some.         
-      intros [(? & ?) | (? & ITH) ]; subst; simpl; try lia.
-      { eapply BB in NTH; eauto. simpl in NTH. lia. }
-      eapply BB in ITH; eauto. lia.
-  Qed.
-
-  Lemma upd_rp_fin_pres rs
-    (FIN: rs_fin rs):
-    rs_fin (upd_rp rs).
-  Proof using.
-    red. destruct FIN; subst; simpl; try by eauto.
-    destruct H; subst; try by eauto.
-  Qed.
-
-  Lemma dequeue_upd_head_spec l τ π q h ph vh (nxh: loc) fl:
-    {{{ queue_inv l ∗
-        ith_node h (ph, (vh, nxh)) ∗ 
-        th_phase_frag τ π q ∗ cp_mul π d get_loc_fuel ∗
-        dequeue_resources h fl ph None }}}
-      #(Head q_sq) <- #nxh @τ
-    {{{ RET #(); th_phase_frag τ π q ∗ dequeue_resources (h + 1) fl nxh (Some h) ∗
-                   ∃ i r b, ith_read i r (h + 1) ∗ ⌜ r <= h ⌝ ∗
-                               br_lb b ∗
-                               (⌜ b < r ⌝ -∗ (ith_rp i rs_canceled ∨ ith_rp i (rs_proc (Some rsp_completed)))) }}}.
-  Proof using.
-    simpl.
-    iIntros (Φ) "([#QAT #INV] & #HTH & PH & CPS & DR) POST".
-    iInv "INV" as "(%hq & %h_ & %t & %br & %fl_ & %rop & %od_ & %hist & %ohv & inv)" "CLOS".
-    iEval (rewrite /queue_inv_inner) in "inv".
-    iDestruct "inv" as "(>HQ & >QI & >DANGLE & OHV & >%ORDER & >AUTHS & >ROP & >RHIST & >%RH_WF & >#OLDS & >RH & >DQ)".
-    iDestruct "DQ" as "[(% & DR') | TOK]".
-    { by iDestruct (dequeue_resources_excl with "[$] [$]") as "?". }
-    iDestruct (dequeue_resources_auth_agree with "[$] [$]") as %[<- <-]. 
-    iDestruct (dequeue_resources_dangle_agree with "[$] [$]") as %->.
-
-    iClear "INV QAT".
-
-    (* TODO: split into lemmas *)
-    iDestruct (hq_auth_lookup with "[$] [$]") as %HTH.
-    iAssert (⌜ t ≠ h ⌝)%I as %NEMPTY.
-    { iIntros (->). iDestruct (queue_interp_cur_empty with "[$]") as %NO.
-      specialize (NO 0). rewrite Nat.add_0_r in NO. congruence. }
-
-    rewrite /dangle_interp. iDestruct "DANGLE" as "(DAUTH & [_ | (% & ?)])"; [| done].
-    rewrite /dequeue_resources. iDestruct "DR" as "(CH & CFL & HEAD' & DFRAG)".
-    rewrite /queue_interp. iDestruct "QI" as "(%T_LEN &  HNIS & %pt & TAIL & TLI & %LL & HEAD & BR & FL)".
-    rewrite HTH. iEval (simpl) in "HEAD".
-
-    iCombine "HEAD HEAD'" as "HEAD". 
-    iApply sswp_MU_wp; [done| ].
-    iApply (wp_store with "[$]"). iIntros "!> [HEAD HEAD']".
-    MU_by_burn_cp. iApply wp_value.
-
-    iMod (dangle_update _ _ (Some h) with "[$] [$]") as "[DAUTH DFRAG]".
-
-    iAssert (|==> auths (h + 1) t br fl ∗ @me_exact _ q_me_h (h + 1))%I with "[CH AUTHS]" as "UPD".
-    { rewrite /auths. iDestruct "AUTHS" as "(AUTH&?&?&?)". iFrame.
-      iApply (me_update with "AUTH CH"). lia. }
-    iMod "UPD" as "[AUTHS CH]".
-
-    iApply "POST". iFrame.
-
-    iAssert (queue_interp hq (h + 1) t br fl ∗ hn_interp (ph, (vh, nxh)))%I
-      with "[HNIS TAIL TLI HEAD BR FL]" as "[QI HNI]".
-    { iFrame. rewrite -!bi.sep_assoc.
-      iSplit; [done| ].
-      iFrame "%".
-      pose proof (take_drop_middle _ _ _ HTH) as SPLIT.
-      rewrite -SPLIT.
-      assert (length (take h hq) = h) as H_LEN. 
-      { apply length_take_le. apply lookup_lt_Some in HTH. lia. }
-      rewrite drop_app_length'; [| done]. simpl.
-      rewrite cons_middle app_assoc.
-      rewrite drop_app_length'.
-      2: { rewrite length_app /=. lia. }
-      iDestruct "HNIS" as "[$ $]".
-      rewrite lookup_app_r.
-      2: { rewrite length_app /=. rewrite H_LEN. lia. }
-      rewrite length_app /=. rewrite H_LEN Nat.sub_diag. 
-      rewrite -SPLIT in LL. 
-      apply is_LL_into_drop with (k := h) in LL.
-      rewrite drop_app_length' in LL; [| done].
-      simpl in LL. destruct (drop (S h) hq) eqn:REST.
-      - by subst.
-      - simpl. destruct h0 as [? [??]]. simpl.
-        by destruct LL as [-> ?]. }
-
-    iDestruct (cancel_rop with "[$]") as "#CNC".
-    { red. rewrite Nat.add_1_r. reflexivity. }
-    
-    iDestruct (take_snapshot with "[$]") as "#SHT".
-    iDestruct "SHT" as "(_&_&#BR_LB&_)". 
-
-    rewrite /rop_interp.
-    destruct rop as [n| ]. 
-    - iDestruct ("ROP" with "[//]") as "(%r & %rp & READ_ & RP & ROP)".      
-      destruct RH_WF as (n' & DOM & [? | [=]] & RH_WF); [done| ]. subst n'. 
-      iMod (read_hist_wf_bump with "[$] [RP]") as "(%r' & %rp' & RHIST & #READ & %RH_WF' & RP & %READ_BOUND)".
-      { eexists. eauto. }
-      { rewrite DOM dom_max_set_fold. iFrame. }
-      rewrite DOM dom_max_set_fold. 
-      iDestruct (ith_read_agree with "READ READ_") as %<-.
-      iFrame "READ". iFrame "%". iFrame "BR_LB". 
-      rewrite -(bi.sep_True' ( ⌜ _ ⌝ -∗ _ )%I). iApply fupd_frame_l. iSplit.
-      { iIntros (LT). iDestruct "ROP" as "[SAFE | [-> _]]".
-        2: { iFrame. }
-        iDestruct "SAFE" as "[FROM_HEAD | [FROM_DANGLE | FROM_BR]]".
-        - iDestruct "FROM_HEAD" as "[-> [-> | (-> & -> & ?)]]".
-          + simpl. iFrame. 
-          + lia. 
-        - iDestruct "FROM_DANGLE" as "[(-> & -> & %X) ?]".
-          clear -X. by destruct X. 
-        - iDestruct "FROM_BR" as "([-> ->] & ->)". lia. } 
-
-      iClear "HTH CPS".
-      iMod ("CLOS" with "[-]") as "_"; [| done].
-      iFrame "QI AUTHS OHV HQ RH DAUTH TOK RHIST". iNext.
-      iExists _. rewrite Nat.add_sub. rewrite HTH /=.
-      
-      iSplitL "HNI". 
-      { iRight. by iFrame. }
-      iSplit.
-      { iPureIntro. red. red in ORDER. repeat split; try lia. }
-      rewrite DOM dom_max_set_fold in RH_WF'.
-      iFrame "%". 
-      iSplit.
-      2: { iApply old_rps_olds.
-           iDestruct (old_rps_olds with "OLDS") as "foo". 
-           by rewrite delete_insert_delete. }
-      rewrite /rop_interp. iIntros (i_ [=]). subst i_. 
-
-      iFrame "READ_ RP". 
-      iDestruct "ROP" as "[[HEAD | [DANGLE | FL]] | CANCEL_WITNESS]".
-      + iDestruct "HEAD" as "(-> & [-> | (-> & -> & TOK)])".
-        * iRight. simpl. by iFrame "#∗".
-        * iLeft. iRight. iLeft. iFrame.
-          iPureIntro. split.
-          ** split; [lia | done].
-          ** simpl. done. 
-      + iDestruct "DANGLE" as "((_ & _ & %) & _)". by destruct H.
-      + iDestruct "FL"as "([-> ->] & ->)". 
-        iLeft. rewrite /safe_read.
-        repeat iRight. done.
-      + iDestruct "CANCEL_WITNESS" as "(-> & CW)".
-        iRight. by iFrame.
-    - destruct RH_WF as (n & DOM & [? | [=]] & RH_WF).
-      destruct (hist !! n) as [[[??]?] | ] eqn:NTH. 
-      2: { apply not_elem_of_dom in NTH. rewrite DOM in NTH.
-           rewrite elem_of_set_seq in NTH. lia. }
-      iDestruct (big_sepM_lookup  with "OLDS") as "RP".
-      { simpl. apply NTH. } 
-      iDestruct "RP" as "(%rp & RP & %FIN & #LB)".
-      iDestruct (ith_rp_hist_compat with "[$] [$]") as %(? & ? & LE').
-      rewrite NTH in H0. inversion H0. subst x. simpl in *.
-
-      iDestruct (read_hist_get hist n with "RHIST") as "#READ".
-      { rewrite NTH. repeat f_equal. }
-      
-      iMod (read_hist_wf_bump with "[$] [RP]") as "(%r' & %rp' & RHIST & #READ' & %RH_WF' & RP_ & %READ_BOUND)".
-      { eexists. eauto. }
-      { rewrite DOM dom_max_set_fold. iFrame "RP". }
-      rewrite DOM dom_max_set_fold.
-      iDestruct (ith_read_agree with "READ READ'") as %->.
-      iFrame "% READ' BR_LB".
-      rewrite -(bi.sep_True' ( ⌜ _ ⌝ -∗ _ )%I). iApply fupd_frame_l. iSplit.
-      { iIntros (LT). destruct FIN as [-> | [-> | ->]].
-        all: try by iFrame.
-        iDestruct (br_lb_bound with "[$] [$]") as %?. lia. }
-
-      iMod ("CLOS" with "[-]") as "_"; [| done].
-      iFrame "QI AUTHS OHV HQ RH DAUTH TOK RHIST". iNext.
-      iExists _. rewrite Nat.add_sub. rewrite HTH /=.
-      
-      iSplitL "HNI". 
-      { iRight. by iFrame. }
-      iSplit.
-      { iPureIntro. red. red in ORDER. repeat split; try lia. }
-      rewrite DOM dom_max_set_fold in RH_WF'.
-      (* do 2 (rewrite decide_False in RH_WF'; [| destruct FIN as [->| [->| ->]]; done]). *)
-      destruct RH_WF as (SEQ &  BB). 
-      Unshelve. 2: exact None. 
-      rewrite bi.sep_assoc.      
-      iSplitR.
-      2: { (* TODO: make a lemma? *)
-        rewrite /old_rps. simpl.
-        rewrite -insert_delete_insert.         
-        rewrite insert_union_singleton_l big_sepM_union.
-        2: { apply map_disjoint_dom. rewrite dom_insert_L. set_solver. }
-        iSplitL.
-        2: { iApply (big_sepM_subseteq with "[$]"). apply delete_subseteq. }
-        rewrite big_sepM_singleton. iFrame. iFrame "% #".
-        iPureIntro. by apply upd_rp_fin_pres. }
-      rewrite /rop_interp. iSplit. 
-      { iIntros (i_ [=]). }
-
-      (* TODO: make a lemma *)
-      rewrite /read_hist_wf.
-      iPureIntro. 
-
-      exists n. split; [| split; [| split]]. 
-    + rewrite dom_insert_L. apply mk_is_Some, elem_of_dom in NTH. set_solver.
-    + tauto. 
-    + intros ?????. rewrite !lookup_insert_Some.
-      intros [(? & ?) | (? & ITH) ] [(? & ?) | (? & JTH) ]; subst; simpl in *; try lia.
-      * apply mk_is_Some, elem_of_dom in JTH.
-        rewrite DOM elem_of_union elem_of_set_seq elem_of_singleton in JTH. lia.
-      * eapply SEQ in H1; eauto. done.
-      * eapply SEQ; eauto.
-    + intros ??. rewrite lookup_insert_Some.         
-      intros [(? & ?) | (? & ITH) ]; subst; simpl; try lia.
-      eapply BB in ITH; eauto. simpl in ITH. lia.
-  Qed.
-
-  Definition dequeue_fuel := 100.    
-
-  Lemma check_BR_spec l τ π q h fl ph ndh i r b0
-    (READ_BOUND: r <= h):
-    {{{ queue_inv l ∗
-        ith_node h (ph, ndh) ∗
-        dequeue_resources (h + 1) fl ndh.2 (Some h) ∗ 
-        th_phase_frag τ π q ∗ cp_mul π d get_loc_fuel ∗
-        ith_read i r (h + 1) ∗ br_lb b0
-    }}}
-      ! #(BeingRead q_sq) @τ
-    {{{ (pbr: loc), RET #pbr; th_phase_frag τ π q ∗
-            dequeue_resources (h + 1) fl ndh.2 (if (decide (pbr = ph)) then Some h else None) ∗
-            (⌜ pbr = ph ⌝ ∨ 
-             ⌜ pbr ≠ ph ⌝ ∗ hn_interp (ph, ndh)) ∗
-            ∃ b' ndbr', br_lb b' ∗ ⌜ b0 <= b' ⌝ ∗ ith_node b' (pbr, ndbr')
-    }}}.
-  Proof using.
-    iIntros (Φ) "([#QAT #INV] & #HTH & DR& PH & CPS & #READ & #BR0) POST".
-    iInv "INV" as "(%hq & %h_ & %t & %br & %fl_ & %rop & %od_ & %hist & %ohv & inv)" "CLOS".
-    iEval (rewrite /queue_inv_inner) in "inv".
-    iDestruct "inv" as "(>HQ & >QI & >DANGLE & OHV & >%ORDER & >AUTHS & >ROP & >RHIST & >%RH_WF & >#OLDS & >RH & >DQ)".
-    iDestruct "DQ" as "[(% & DR') | TOK]".
-    { by iDestruct (dequeue_resources_excl with "[$] [$]") as "?". }
-    iDestruct (dequeue_resources_auth_agree with "[$] [$]") as %[<- <-]. 
-    iDestruct (dequeue_resources_dangle_agree with "[$] [$]") as %->.
-
-    iClear "INV QAT".
-
-    (* TODO: split into lemmas *)
-    iDestruct (hq_auth_lookup with "[$] [$]") as %HTH.
-    iAssert (⌜ t ≠ h ⌝)%I as %NEMPTY.
-    { iIntros (->). red in ORDER. lia. }
-
-    rewrite /dangle_interp. iDestruct "DANGLE" as "(DAUTH & [% | (_ & HNI)])"; [done| ].
-    rewrite Nat.add_sub HTH /=. 
-    rewrite /dequeue_resources. iDestruct "DR" as "(CH & CFL & HEAD' & DFRAG)".
-    rewrite /queue_interp. iDestruct "QI" as "(%T_LEN &  HNIS & %pt & TAIL & TLI & %LL & HEAD & BR & FL)".
-    iDestruct "BR" as "(%nbr & %BRTH & BR)". destruct nbr as [pbr nbr].
-
-    iApply sswp_MU_wp; [done| ]. 
-    iApply (wp_load with "BR"). iIntros "!> BR".
-    MU_by_burn_cp. iApply wp_value.
-
-    iApply "POST". iFrame.
-
-    iDestruct (br_lb_bound with "BR0 AUTHS") as %BR0. 
-    iDestruct (take_snapshot with "[$]") as "#SHT".
-    iDestruct (hq_auth_get_ith with "HQ") as "#BRTH'".
-    { apply BRTH. }
-    iFrame "BRTH'". 
-
-    iAssert (queue_interp hq (h + 1) t br fl)%I
-      with "[HNIS TAIL TLI HEAD BR FL]" as "QI".
-    { by iFrame. }
-    iAssert (br_lb br ∗ ⌜b0 ≤ br⌝)%I as "$".
-    { iSplit; [| done].
-      iDestruct "SHT" as "(?&?&?&?)". done. }
-
-    simpl.
-    destruct (decide (pbr = ph)) as [-> | NEQ].
-    -
-      iFrame. 
-      iMod ("CLOS" with "[-]") as "_".
-      { iFrame "#∗ %". iNext.
-        rewrite Nat.add_sub HTH /=.
-        iRight. by iFrame. }
-      iModIntro. by iLeft.
-    - iDestruct (ith_read_hist_compat with "[$] [$]") as %(b & p & READ & INCR_BOUND). 
-      iMod (dangle_update _ _ None with "[$] [$]") as "[DAUTH DFRAG]".
-      iFrame.      
-      iApply fupd_or. iRight. iFrame "HNI".
-      rewrite -(bi.sep_True' ⌜ _ ≠ _ ⌝%I). iApply fupd_frame_l. iSplit; [done| ].
-      iMod ("CLOS" with "[-]") as "_"; [| done]. 
-
-      rewrite /rop_interp.
-      destruct rop.
-      2: { iFrame "#∗ %". iNext. iSplitR.
-           { by iLeft. }
-           rewrite /rop_interp. by iIntros (??). }
-      
-      iDestruct ("ROP" with "[//]") as "(%r_ & %rp & READ_ & RP & ROP)".
-      iDestruct (ith_read_hist_compat with "[$] READ_") as %(?&? & READ' & _). 
-
-      iFrame. iFrame "OLDS".
-      iNext. iSplitR.
-      { by iLeft. }
-      iSplit; [done| ]. iSplit; [| done]. 
-      rewrite /rop_interp.
-      iIntros (i' [=]). subst n.
-      iDestruct "ROP" as "[SAFE | $]".
-      2: { iFrame "#∗". }
-
-      destruct (decide (i' = i)). 
-      { subst. rewrite {1}/safe_read. rewrite Nat.add_sub.
-        iFrame "READ_". 
-        iDestruct "SAFE" as "[FROM_HEAD | [FROM_DANGLE | FROM_BR]]".
-        - iFrame.
-        - iDestruct "FROM_DANGLE" as "[(-> & -> & _) ?]".
-          congruence.
-        - iFrame. }
-
-      assert (i < i') as NEW.
-      { red in RH_WF. destruct RH_WF as (n' & DOM & [? | [=]] & RH_WF); [done| ].
-        subst i'.
-        apply mk_is_Some, elem_of_dom in READ. rewrite DOM elem_of_set_seq in READ.
-        lia. }
-      clear n.
-      
-      assert (h + 1 <= r_) as READ'_BOUND.
-      { red in RH_WF. destruct RH_WF as (n' & DOM & [? | [=]] & RH_WF); [done| ].
-        subst. 
-        apply proj1 in RH_WF. eapply RH_WF in NEW; eauto. simpl in NEW. lia. }
-      iFrame "READ_".
-      rewrite {1}/safe_read.
-      iDestruct "SAFE" as "[FROM_HEAD | [FROM_DANGLE | FROM_BR]]".
-      + iFrame.
-      + iDestruct "FROM_DANGLE" as "[(-> & -> & _) ?]". lia.
-      + iFrame.
-  Qed.
-
-  Lemma read_FL_spec τ π l h q fl nd od:
-  {{{ queue_inv l ∗ dequeue_resources h fl nd od ∗
-      cp π d ∗ th_phase_frag τ π q }}}
-    ! #(FreeLater q_sq) @τ
-  {{{ (pfl: loc), RET (#pfl);
-      ∃ ndfl, ith_node fl (pfl, ndfl) ∗ 
-      dequeue_resources h fl nd od ∗ th_phase_frag τ π q }}}.
-  Proof using.
-    iIntros (Φ) "([#QAT #INV] & DR & CPS & PH) POST".
-    iInv "INV" as "(%hq & %h_ & %t & %br & %fl_ & %rop & %od_ & %hist & %ohv & inv)" "CLOS".
-    iEval (rewrite /queue_inv_inner) in "inv".
-    iDestruct "inv" as "(>HQ & >QI & >DANGLE & OHV & >%ORDER & >AUTHS & >ROP & >RHIST & >%RH_WF & >#OLDS & >RH & >DQ)".
-    iDestruct "DQ" as "[(% & DR') | TOK]".
-    { by iDestruct (dequeue_resources_excl with "[$] [$]") as "?". }
-    iDestruct (dequeue_resources_auth_agree with "[$] [$]") as %[<- <-].
-    rewrite /queue_interp. iDestruct "QI" as "(%T_LEN &  HNIS & %pt & TAIL & TLI & %LL & HEAD & BR & FL)".
-    iDestruct "FL" as "(%x & %FLTH & FL & HNI_FL)". 
-    iDestruct (hq_auth_get_ith with "[$]") as "#FLTH"; [by eauto| ].
-    iApply sswp_MU_wp; [done| ].     
-    iApply (wp_load with "FL"). iIntros "!> FL".
-    rewrite cp_mul_1. 
-    MU_by_burn_cp. iApply wp_value.
-    iMod ("CLOS" with "[-POST DR PH]") as "_".
-    { iFrame. iFrame "OLDS". done. }
-    iModIntro. iApply "POST". iFrame.
-    destruct x. iFrame "FLTH".     
-  Qed.
-
   (* TODO: also holds if h is not in the hist queue (e.g. initially) *)
   Lemma queue_interp_ph_neq_pfl' (hq: HistQueue) h t br fl (ptr: loc):
     queue_interp hq h t br fl -∗ ⌜ exists nd, hq !! h = Some (ptr, nd) ⌝ -∗
@@ -999,365 +439,4 @@ Section SimpleQueue.
     by iDestruct (hn_interp_ptr_excl with "[$] [$]") as "?".
   Qed.
 
-  Lemma get_to_free_spec 
-    l τ π q h fl (ph: loc) ndh i r b
-    (READ_BOUND: r <= h):
-    {{{ queue_inv l ∗
-        ith_node h (ph, ndh) ∗
-        dequeue_resources (h + 1) fl ndh.2 (Some h) ∗ 
-        th_phase_frag τ π q ∗ cp_mul π d (get_loc_fuel + get_loc_fuel + get_loc_fuel) ∗
-        ith_read i r (h + 1) ∗
-        br_lb b ∗ (⌜ b < r ⌝ -∗ (ith_rp i rs_canceled ∨ ith_rp i (rs_proc (Some rsp_completed))))
-    }}}
-      get_to_free q_sq #ph @ τ
-    {{{ (to_free: loc), RET #to_free;
-        ∃ hn fl', hn_interp (to_free, hn) ∗ th_phase_frag τ π q ∗
-                    dequeue_resources (h + 1) fl' ndh.2 None }}}.
-  Proof using.
-    simpl.
-    iIntros (Φ) "([#QAT #INV] & #HTH & DR& PH & CPS & #READ & #BR0 & #NO_FL) POST".
-    rewrite /get_to_free. destruct q_sq eqn:Q_SQ. 
-    pure_steps. 
-    
-    split_cps "CPS" get_loc_fuel.
-    wp_bind (! _)%E. 
-    replace BeingRead0 with (BeingRead q_sq) by (by rewrite Q_SQ). 
-    iApply (check_BR_spec with "[-POST CPS]").
-    { apply READ_BOUND. }
-    { iFrame "#∗". }
-    iIntros "!> %pbr (PH & DR & RES)".
-    iDestruct "RES" as "(RES & %b1 & %ndbr1 & #BR1 & %LEb & #BRTH1)". 
-
-    wp_bind (_ = _)%E.
-    iApply sswp_MU_wp; [done| ].
-    iApply sswp_pure_step.
-    { set_solver. }
-    MU_by_burn_cp. iApply wp_value.
-
-    iDestruct "RES" as "[%PTR_EQ | [%NEQ HNI]]".
-    2: { rewrite bool_decide_false; [| set_solver]. rewrite decide_False; [| done].
-         pure_steps. iApply "POST". iFrame. }
-
-    rewrite PTR_EQ. 
-
-    rewrite bool_decide_true; [| set_solver]. rewrite decide_True; [| done].
-    pure_steps.
-
-    wp_bind (! _)%E.
-    split_cps "CPS" 1. rewrite -cp_mul_1.
-    replace FreeLater0 with (FreeLater q_sq) by (by rewrite Q_SQ). 
-    iApply (read_FL_spec with "[-POST CPS]").
-    { iFrame "#∗". }
-    iIntros "!> %pfl (%ndfl & #FLTH & DR & PH)".
-
-    wp_bind (Rec _ _ _)%E. pure_steps.
-
-    wp_bind (_ <- _)%E.
-
-    iInv "INV" as "(%hq & %h_ & %t & %br & %fl_ & %rop & %od_ & %hist & %ohv & inv)" "CLOS".
-    iEval (rewrite /queue_inv_inner) in "inv".
-    iDestruct "inv" as "(>HQ & >QI & >DANGLE & OHV & >%ORDER & >AUTHS & >ROP & >RHIST & >%RH_WF & >#OLDS & >RH & >DQ)".
-    iDestruct "DQ" as "[(% & DR') | TOK]".
-    { by iDestruct (dequeue_resources_excl with "[$] [$]") as "?". }
-    iDestruct (dequeue_resources_auth_agree with "[$] [$]") as %[<- <-]. 
-    iDestruct (dequeue_resources_dangle_agree with "[$] [$]") as %->.
-
-    iClear "INV QAT".
-
-    (* TODO: split into lemmas *)
-    iDestruct (hq_auth_lookup with "[$] HTH") as %HTH.
-    iAssert (⌜ t ≠ h ⌝)%I as %NEMPTY.
-    { iIntros (->). red in ORDER. lia. }
-
-    iPoseProof (queue_interp_dangle_neq_pfl' _ _ _ _ _ ph with "QI [DANGLE]") as "#PFL_NEQ_D".
-    { by rewrite Nat.add_sub. }
-
-    rewrite /dangle_interp. iDestruct "DANGLE" as "(DAUTH & [% | (_ & HNI)])"; [done| ].
-    rewrite Nat.add_sub HTH /=. 
-    rewrite /dequeue_resources. iDestruct "DR" as "(CH & CFL & HEAD' & DFRAG)".
-
-    
-    rewrite /queue_interp. iDestruct "QI" as "(%T_LEN &  HNIS & %pt & TAIL & TLI & %LL & HEAD & BR & FL)".
-    iDestruct "BR" as "(%nbr & %BRTH & BR)".
-    
-    iDestruct (br_lb_bound with "BR1 AUTHS") as %BR1. 
-
-    subst pbr. 
-    destruct nbr as [pbr nbr].
-
-    (* iCombine "HEAD HEAD'" as "HEAD".  *)
-    iApply sswp_MU_wp; [done| ].
-
-    iDestruct "FL" as "(%ndfl_ & %FLTH & FL & HNI_FL)".
-    iDestruct (hq_auth_lookup with "[$] FLTH") as %FLTH_.
-    rewrite FLTH in FLTH_. inversion FLTH_. subst ndfl_. clear FLTH_. 
-    iApply (wp_store with "FL"). iIntros "!> FL".
-    MU_by_burn_cp. iApply wp_value.
-
-    iMod (dangle_update _ _ None with "[$] [$]") as "[DAUTH DFRAG]".
-    iAssert (|==> auths (h + 1) t br h ∗ @me_exact _ q_me_fl h)%I with "[CFL AUTHS]" as "UPD".
-    { rewrite /auths. iDestruct "AUTHS" as "(?&?&?&A)". iFrame.
-      iApply (me_update with "A CFL"). red in ORDER. lia. }
-    iMod "UPD" as "[AUTHS CFL]".
-
-    iDestruct (br_lb_bound with "BR0 [$]") as %BR0. 
-    iAssert (queue_interp hq (h + 1) t br h)%I
-      with "[HNIS TAIL TLI HEAD BR FL HNI]" as "QI".
-    { iFrame. 
-      iSplit; [done| ].
-      iFrame "%". iFrame. } 
-
-    rewrite /rop_interp.
-    destruct rop. 
-    - iDestruct ("ROP" with "[//]") as "(%r_ & %rp & READ_ & RP & ROP)".
-      iDestruct (ith_read_hist_compat with "[$] READ_") as %(?&? & READ' & _). 
-      iDestruct (ith_read_hist_compat with "[$] READ") as %(?&? & READ & BB).
-      iDestruct (hq_auth_lookup with "[$] BRTH1") as %BRTH1.
-      
-      iAssert (dequeue_resources (h + 1) h ndh.2 None)%I with "[CH CFL HEAD' DFRAG]" as "DR".
-      { iFrame. }
-
-      iMod ("CLOS" with "[-POST CPS PH DR HNI_FL]") as "_".
-      { iFrame. iExists _. iNext. iSplitR.
-        { by iLeft. }        
-        iFrame "%". iFrame "OLDS". 
-        iSplit; cycle 1.
-        - rewrite /rop_interp.
-          iIntros (i' [=]). subst n.
-          iDestruct "ROP" as "[SAFE | $]".
-          2: { iFrame. }
-          iFrame "READ_".
-          
-          destruct (decide (i' = i)). 
-          { subst. rewrite {1}/safe_read. rewrite Nat.add_sub.
-            iDestruct "SAFE" as "[FROM_HEAD | [FROM_DANGLE | FROM_BR]]".
-            - iFrame.
-            - iDestruct "FROM_DANGLE" as "[(-> & -> & _) ->]".
-              iFrame "RP". 
-              iLeft. rewrite /safe_read. rewrite Nat.add_sub.
-              do 2 iRight. by iFrame. 
-            - iDestruct "FROM_BR" as "([-> ->] & ->)". 
-              rewrite READ in READ'. inversion READ'. subst r x1 x2.
-              apply Nat.le_lteq in BR0 as [BR0 | ->].
-              { iSpecialize ("NO_FL" with "[//]"). iExFalso.
-                iAssert (∃ rp', ith_rp i rp' ∗ ⌜ rp' = rs_canceled \/ rp' = (rs_proc (Some rsp_completed))⌝)%I as "(%rp' & RP' & %RP')".
-                { iDestruct "NO_FL" as "[$|$]"; set_solver. }
-                iDestruct (ith_rp_le with "RP RP'") as %CM.
-                exfalso. clear -RP' CM.
-                inversion CM; destruct RP' as [-> | ->]; try done.
-                subst. inversion RSP. by subst. }
-              rename x into bi.
-              red in RH_WF.
-              destruct RH_WF as (n' & DOM & [? | [=]] & SEQ & BB'); [done| ].
-              subst n'.
-              pose proof READ as EQ%BB'. simpl in EQ.
-              assert (bi = h + 1) as -> by lia.  clear BB EQ.
-              assert (b1 = fl) as -> by lia.
-              rewrite BRTH in BRTH1. inversion BRTH1. subst pbr ndbr1.
-              iDestruct ("PFL_NEQ_D" with "[] []") as "?".
-              { eauto. }
-              { eauto. }
-              done. }
-          
-          assert (i < i') as NEW.
-          { red in RH_WF. destruct RH_WF as (n' & DOM & [? | [=]] & RH_WF); [done| ].
-            subst i'.
-            apply mk_is_Some, elem_of_dom in READ. rewrite DOM elem_of_set_seq in READ.
-            lia. }
-          clear n.
-
-          assert (h + 1 <= r_) as READ'_BOUND.
-          { red in RH_WF. destruct RH_WF as (n' & DOM & [? | [=]] & RH_WF); [done| ].
-            apply proj1 in RH_WF. eapply RH_WF in NEW; eauto. simpl in NEW. lia. }
-          rewrite {1}/safe_read.
-          iDestruct "SAFE" as "[FROM_HEAD | [FROM_DANGLE | FROM_BR]]".
-          + iFrame.
-          + iDestruct "FROM_DANGLE" as "[(-> & -> & _) ?]". lia.
-          + iFrame.
-            iDestruct "FROM_BR" as "([% %] & ?)". subst.
-            red in ORDER. lia.
-        - rewrite /hq_state_wf. iPureIntro.
-          red in ORDER. lia. }
-
-      iModIntro. wp_bind (Rec _ _ _)%E. pure_steps.
-      iApply "POST". iFrame. 
-    - 
-      iAssert (dequeue_resources (h + 1) h ndh.2 None)%I with "[CH CFL HEAD' DFRAG]" as "DR".
-      { iFrame. }
-
-      iMod ("CLOS" with "[-POST CPS PH DR HNI_FL]") as "_".
-      { iFrame. iExists _. iNext. iSplitR.
-        { by iLeft. }
-        iFrame "% OLDS".
-        iSplit; cycle 1.
-        - rewrite /rop_interp. by iIntros (??). 
-        - rewrite /hq_state_wf. iPureIntro.
-          red in ORDER. lia. }
-
-      iModIntro. wp_bind (Rec _ _ _)%E. pure_steps.
-      iApply "POST". iFrame. 
-  Qed.
-
-  Lemma free_el_spec τ π q ptr nd:
-    {{{ th_phase_frag τ π q ∗ cp_mul π d get_loc_fuel ∗ 
-        hn_interp (ptr, nd) }}}
-      free_el #ptr @ τ
-    {{{ v, RET v; th_phase_frag τ π q }}}.
-  Proof using. Admitted. 
-  
-  Lemma dequeue_spec l (τ: locale heap_lang) (π: Phase) (q: Qp):
-    {{{ queue_inv l ∗ dequeue_token ∗ 
-        th_phase_frag τ π q ∗ cp_mul π d dequeue_fuel }}}
-      dequeue q_sq l @ τ
-    {{{ (v: val), RET v; th_phase_frag τ π q ∗ dequeue_token }}}.
-  Proof using.
-    simpl. iIntros (Φ) "([#QAT #INV] & TOK & PH & CPS) POST".
-    rewrite /dequeue. destruct q_sq eqn:Q_SQ.
-    pure_steps.
-
-    wp_bind (! _)%E.
-    iInv "INV" as "(%hq & %h & %t & %br & %fl & %rop & %od & %hist & %ohv & inv)" "CLOS".
-    iEval (rewrite /queue_inv_inner) in "inv".
-    iDestruct "inv" as "(>HQ & >QI & >DANGLE & OHV & >%ORDER & >AUTHS & >ROP & >RHIST & >%RH_WF & >#OLDS & >RH & >DQ)".
-    
-    iApply sswp_MU_wp; [done| ].
-    iDestruct (access_queue_ends with "[$] [$]") as "(%ph & %pt & HEAD & TAIL & HT & CLOS')".
-    replace Head0 with (Head q_sq) by (by rewrite Q_SQ).
-    iApply (wp_load with "HEAD"). iIntros "!> HEAD".
-    iDestruct "DQ" as "[[%ph_ DR] | TOK']".
-    2: { by iDestruct (dequeue_token_excl with "[$] [$]") as "?". }
-    iDestruct (dequeue_res_head_agree with "DR [$]") as %<-. 
-    iDestruct (dequeue_resources_dangle_agree with "DR [$]") as %->.
-    iDestruct ("CLOS'" with "[$] [$]") as "(HQ & QI)".
-    MU_by_burn_cp. iApply wp_value.
-
-    iMod ("CLOS" with "[-POST CPS PH DR]") as "_".
-    { iFrame. by iFrame "OLDS". }
-    iModIntro.
-
-    (* TODO: do we need to keep track of previous values at this point? *)
-    clear t br ohv ORDER hq.
-    iClear "OLDS". 
-    clear pt rop RH_WF hist.
-
-    wp_bind (Rec _ _ _)%E. pure_steps. 
-    
-    wp_bind (! _)%E.
-    iInv "INV" as "(%hq & %h_ & %t & %br & %fl_ & %rop & %od_ & %hist & %ohv & inv)" "CLOS".
-    iEval (rewrite /queue_inv_inner) in "inv".
-    iDestruct "inv" as "(>HQ & >QI & >DANGLE & OHV & >%ORDER & >AUTHS & >ROP & >RHIST & >%RH_WF & >#OLDS & >RH & >DQ)".
-    iApply sswp_MU_wp; [done| ].
-    iDestruct (access_queue_ends with "[$] [$]") as "(%ph_ & %pt & HEAD & TAIL & #HT & CLOS')".
-    replace Tail0 with (Tail q_sq) by (by rewrite Q_SQ).
-    iApply (wp_load with "[$]"). iIntros "!> TAIL".
-    iDestruct (dequeue_res_head_agree with "DR [$]") as %->. 
-    iDestruct (dequeue_resources_auth_agree with "DR [$]") as %[<- <-].
-    iDestruct (take_snapshot with "[$]") as "#SHT".
-    iDestruct "DQ" as "[(% & DR') | TOK]".
-    { by iDestruct (dequeue_resources_excl with "DR DR'") as "?". }
-
-    iDestruct ("CLOS'" with "[$] [$]") as "(HQ & QI)".
-    MU_by_burn_cp. iApply wp_value.
-    iMod ("CLOS" with "[-POST CPS PH DR]") as "_".
-    { iFrame. by iFrame "OLDS". }
-    iModIntro.
-
-    (* TODO: do we need to keep track of previous values at this point? *)
-    (* clear br hob od ohv ORDER SAFE_BR hq. *)
-    iClear "OLDS SHT". 
-    clear ohv hist hq RH_WF od_ (* ORDER *) rop (* br *).    
-
-    wp_bind (_ = _)%E.
-    iApply sswp_MU_wp; [done| ].
-    iApply sswp_pure_step.
-    { set_solver. }
-    MU_by_burn_cp. iApply wp_value.
-
-    (* destruct bool_decide. *)
-    iDestruct "HT" as "[[%GE <-] | (%NEMPTY & %ndh & #HTH)]". 
-    { assert (t = h) as ->.
-      { red in ORDER. lia. }
-      rewrite bool_decide_true; [| done]. 
-      iApply sswp_MU_wp_fupd; [done| ]. 
-      iInv "INV" as "(%hq & %h_ & %t & %br' & %fl_ & %rop & %od_ & %hist & %ohv & inv)" "CLOS".
-      iEval (rewrite /queue_inv_inner) in "inv".
-      iDestruct "inv" as "(>HQ & >QI & >DANGLE & OHV & >%ORDER' & >AUTHS & >ROP & >RHIST & >%RH_WF & >#OLDS & >RH & >DQ)".
-      iModIntro.
-      iApply sswp_pure_step; [done| ].
-      do 2 iNext. MU_by_burn_cp.
-      iDestruct "DQ" as "[(% & DR') | TOK]".
-      { by iDestruct (dequeue_resources_excl with "[$] [$]") as "?". }
-      iDestruct (dequeue_resources_auth_agree with "[$] [$]") as %[-> ->]. 
-      iMod ("CLOS" with "[-POST CPS PH TOK]") as "_".
-      { iFrame. by iFrame "OLDS". }
-      iModIntro. pure_steps.
-      iApply "POST". iFrame. }
-
-    rewrite bool_decide_false; [| set_solver]. pure_steps.
-    split_cps "CPS" get_loc_fuel; [cbv; lia| ].  
-    iApply (get_head_val_spec with "[-POST CPS]").
-    { iFrame "#∗". }
-    iIntros "!> [PH DR]".
-    wp_bind (Rec _ _ _)%E. pure_steps.
-
-    destruct ndh as [vh nxh]. simpl.
-    wp_bind (_ <- _)%E.
-    replace OldHeadVal0 with (OldHeadVal q_sq) by (by rewrite Q_SQ).
-    split_cps "CPS" get_loc_fuel; [cbv; lia| ].     
-    iApply (update_ohv_spec with "[$QAT $PH $CPS' $INV]").
-    iIntros "!> PH".
-    wp_bind (Rec _ _ _)%E. pure_steps.
-
-    split_cps "CPS" get_loc_fuel; [cbv; lia| ].
-    iApply (get_head_next_spec with "[-POST CPS]").
-    { iFrame "#∗". }
-    iIntros "!> [PH DR]". simpl.
-
-    wp_bind (_ <- _)%E.
-    split_cps "CPS" get_loc_fuel; [cbv; lia| ].
-    iApply (dequeue_upd_head_spec with "[$QAT $CPS' $PH $INV $HTH $DR]").
-    iIntros "!> (PH & DR & (%i & %r & %b & #ITHR & %BR & #TOKS))".
-
-    wp_bind (Rec _ _ _)%E. do 3 pure_step_cases.
-    fold (get_to_free (SQ Head0 Tail0 BeingRead0 FreeLater0 OldHeadVal0)).
-    rewrite -Q_SQ. 
-    wp_bind (get_to_free _ _)%E.         
-    split_cps "CPS" (3 * get_loc_fuel); [cbv; lia| ].
-    iApply (get_to_free_spec with "[-POST CPS]").
-    { apply BR. }
-    { iFrame "#∗". }
-    
-    iIntros "!> %to_free (%hfr & %fl' & HNFR & PH & DR)".
-    wp_bind (Rec _ _ _)%E. pure_steps.
-    wp_bind (free_el _)%E.
-    split_cps "CPS" get_loc_fuel; [cbv; lia| ].
-    iApply (free_el_spec with "[CPS' PH HNFR]").
-    { iFrame. }
-    iIntros "!> %v PH".
-
-    wp_bind (Rec _ _ _)%E. do 2 pure_step_cases. 
-    iClear "TOKS ITHR HTH". 
-    clear dependent r t hfr to_free br ph b. 
-
-    iApply sswp_MU_wp_fupd; [done| ]. 
-    iInv "INV" as "(%hq & %h_ & %t & %br & %fl_ & %rop & %od & %hist & %ohv & inv)" "CLOS".
-    iEval (rewrite /queue_inv_inner) in "inv".
-    iDestruct "inv" as "(>HQ & >QI & >DANGLE & OHV & >%ORDER & >AUTHS & >ROP & >RHIST & >%RH_WF & >#OLDS & >RH & >DQ)".
-    iDestruct "DQ" as "[(% & DR') | TOK]".
-    { by iDestruct (dequeue_resources_excl with "DR DR'") as "?". }
-    (* iDestruct (dequeue_res_head_agree with "DR [$]") as %->.  *)
-    iDestruct (dequeue_resources_auth_agree with "DR [$]") as %[<- <-].
-    iDestruct (dequeue_resources_dangle_agree with "DR [$]") as %->.
-
-    iModIntro. iApply sswp_pure_step; [done| ]. 
-    MU_by_burn_cp. simpl.
-    iMod ("CLOS" with "[-POST CPS PH TOK]") as "_".
-    { iFrame. by iFrame "OLDS". }
- 
-    iModIntro. pure_steps.
-    iApply "POST". iFrame.
-  Qed.
-
-  Print Assumptions dequeue_spec.
-    
-End SimpleQueue.
+End QueueResources.
