lawyer/nonblocking/examples/dequeue.v
@@ -1,0 +1,931 @@
+From iris.base_logic Require Export gen_heap.
+From iris.proofmode Require Import tactics coq_tactics.
+From iris.bi.lib Require Import fixpoint.
+From trillium.program_logic Require Export weakestpre adequacy ectx_lifting.
+From fairness Require Import utils.
+From lawyer.examples Require Import obls_tactics.
+From lawyer.nonblocking.examples Require Import simple_queue_utils simple_queue.
+From lawyer.obligations Require Import obligations_model obligations_resources obligations_am obligations_em obligations_logic env_helpers.
+From lawyer Require Import sub_action_em program_logic.
+From iris.algebra Require Import auth gmap gset excl excl_auth csum mono_nat.
+From iris.base_logic.lib Require Import invariants.
+
+
+Close Scope Z.
+
+Section Dequeue.
+
+  Context {DegO LvlO LIM_STEPS} {OP: OP_HL DegO LvlO LIM_STEPS}.
+  Context `{EM: ExecutionModel heap_lang M}.
+  Notation "'Degree'" := (om_hl_Degree). 
+  Notation "'Level'" := (om_hl_Level).  
+
+  Context {Σ} {OHE: OM_HL_Env OP EM Σ}.
+  (* Existing Instance OHE.  *)
+  Context {QL: QueueG Σ}.
+
+  Context (d: Degree).
+
+  Definition get_loc_fuel := 5.
+
+  Let hGS: heap1GS Σ := iem_phys _ EM.
+  Existing Instance hGS. 
+
+  Lemma get_head_val_spec Q τ π q h nd fl ph od:
+    {{{ queue_inv Q ∗ ith_node h (ph, nd) ∗ dequeue_resources h fl ph od ∗
+        th_phase_frag τ π q ∗ cp_mul π d get_loc_fuel }}}
+      get_val #ph @τ
+    {{{ RET (nd.1); th_phase_frag τ π q ∗ dequeue_resources h fl ph od }}}.
+  Proof using.
+    simpl. iIntros (Φ) "([#QAT #INV] & #HEADhn & DR & PH & CPS) POST".
+    rewrite /get_val.
+    destruct nd as [v nxt]. simpl.
+    pure_steps.
+    wp_bind (_ +ₗ _)%E.
+    iApply sswp_MU_wp; [done| ].
+    iApply sswp_pure_step; [done| ].
+    MU_by_burn_cp. rewrite loc_add_0. iApply wp_value.
+    iInv "INV" as "(%hq & %h_ & %t & %br & %fl_ & %rop & %od_ & %hist & %ohv & inv)" "CLOS".
+    iEval (rewrite /queue_inv_inner) in "inv".
+    iDestruct "inv" as "(>HQ & >QI & DANGLE & OHV & >%ORDER & >AUTHS & >ROP & RHIST & >%RH_WF & RH & DQ)".
+    iDestruct (dequeue_resources_auth_agree with "[$] [$]") as %[<- <-].
+    iDestruct "DR" as "[HEAD FL]".
+    iDestruct (hq_auth_lookup with "[$] [$]") as %HTH.
+    iAssert (⌜ t ≠ h ⌝)%I as %NEMPTY.
+    { iIntros (->). iDestruct (queue_interp_cur_empty with "[$]") as %NO.
+      specialize (NO 0). rewrite Nat.add_0_r in NO. congruence. } 
+    iDestruct (access_queue with "[$] [$] [$]") as "[HNI CLOS']".
+    { red in ORDER. lia. }
+    rewrite {1}/hn_interp. iDestruct "HNI" as "[VAL NXT]".
+    iApply sswp_MU_wp; [done| ].
+    iApply (wp_load with "VAL"). iIntros "!> VAL". 
+    MU_by_burn_cp. iApply wp_value.
+    iDestruct ("CLOS'" with "[$VAL $NXT]") as "[??]".
+    iMod ("CLOS" with "[-POST PH HEAD FL]") as "_".
+    { by iFrame. }
+    iModIntro. iApply "POST". iFrame.
+  Qed.
+
+  (* TODO: unify with the proof above *)
+  Lemma get_head_next_spec Q τ π q h nd fl ph od:
+    {{{ queue_inv Q ∗ ith_node h (ph, nd) ∗ dequeue_resources h fl ph od ∗
+        th_phase_frag τ π q ∗ cp_mul π d get_loc_fuel }}}
+      get_next #ph @τ
+    {{{ RET #(nd.2); th_phase_frag τ π q ∗ dequeue_resources h fl ph od }}}.
+  Proof using.
+    simpl. iIntros (Φ) "([#QAT #INV] & #HEADhn & DR & PH & CPS) POST".
+    rewrite /get_next.
+    destruct nd as [v nxt]. simpl.
+    pure_steps.
+    wp_bind (_ +ₗ _)%E.
+    iApply sswp_MU_wp; [done| ].
+    iApply sswp_pure_step; [done| ].
+    MU_by_burn_cp. iApply wp_value.
+    iInv "INV" as "(%hq & %h_ & %t & %br & %fl_ & %rop & %od' & %hist & %ohv & inv)" "CLOS".
+    iEval (rewrite /queue_inv_inner) in "inv".
+    iDestruct "inv" as "(>HQ & >QI & DANGLE & OHV & >%ORDER & >AUTHS & >ROP & RHIST & >%RH_WF & RH & DQ)".
+    iDestruct (dequeue_resources_auth_agree with "[$] [$]") as %[<- <-].
+    iDestruct "DR" as "[HEAD FL]".
+    iDestruct (hq_auth_lookup with "[$] [$]") as %HTH.
+    iAssert (⌜ t ≠ h ⌝)%I as %NEMPTY.
+    { iIntros (->). iDestruct (queue_interp_cur_empty with "[$]") as %NO.
+      specialize (NO 0). rewrite Nat.add_0_r in NO. congruence. } 
+    iDestruct (access_queue with "[$] [$] [$]") as "[HNI CLOS']".
+    { red in ORDER. lia. }
+    rewrite {1}/hn_interp. iDestruct "HNI" as "[VAL NXT]".
+    iApply sswp_MU_wp; [done| ].
+    iApply (wp_load with "NXT"). iIntros "!> NXT". 
+    MU_by_burn_cp. iApply wp_value.
+    iDestruct ("CLOS'" with "[$VAL $NXT]") as "[??]".
+    iMod ("CLOS" with "[-POST PH HEAD FL]") as "_".
+    { by iFrame. }
+    iModIntro. iApply "POST". iFrame.
+  Qed.
+
+  Lemma update_ohv_spec τ π q (v: val) l:
+    {{{ queue_inv l ∗ th_phase_frag τ π q ∗ cp_mul π d get_loc_fuel }}}
+      #(OldHeadVal q_sq) <- v @τ
+    {{{ RET #(); th_phase_frag τ π q }}}.
+  Proof using.
+    iIntros (Φ) "([#QAT #INV] & PH & CPS) POST".
+    iInv "INV" as "(%hq & %h & %t & %br & %fl & %rop & %od & %hist & %ohv & inv)" "CLOS".
+    iEval (rewrite /queue_inv_inner) in "inv".
+    iDestruct "inv" as "(>HQ & >QI & DANGLE & OHV & >%ORDER & >AUTHS & >ROP & RHIST & >%RH_WF & RH & DQ)".
+
+    iApply sswp_MU_wp; [done| ].
+    iApply (wp_store with "[$]"). iIntros "!> ?".
+    MU_by_burn_cp. iApply wp_value.
+    iMod ("CLOS" with "[-POST PH]") as "_". 
+    { by iFrame. }
+    by iApply "POST".
+  Qed.
+
+  Lemma is_LL_into_drop hq pt k
+    (LL: is_LL_into hq pt):
+    is_LL_into (drop k hq) pt.
+  Proof using.
+    revert k. induction hq.
+    { intros. by rewrite drop_nil. }
+    intros. destruct k.
+    { by rewrite drop_0. }
+    simpl. apply IHhq.
+    simpl in LL. destruct a as [? [? ?]].
+    destruct hq; try done.
+    destruct h as [? [? ?]]. tauto.
+  Qed.
+
+  Lemma dom_max_set_fold n:
+    set_fold max 0 (set_seq 0 (S n): gset nat) = n.
+  Proof using.
+    clear. induction n.
+    { done. }
+    rewrite set_seq_S_end_union_L.
+    rewrite union_comm_L. 
+    erewrite set_fold_union.
+    2-4: red; lia.
+    simpl. rewrite IHn.
+    rewrite set_fold_singleton. lia.
+  Qed.
+
+  Definition upd_rp rp :=
+    match rp with
+    | rs_init => rs_canceled
+    | rs_proc (Some rsp_going) => rs_proc (Some rsp_protected)
+    | _ => rp
+    end. 
+
+  Lemma upd_rp_rs_step p: rs_step p (upd_rp p).
+  Proof using.
+    destruct p; simpl; try constructor.
+    destruct orsp; simpl; try constructor.
+    destruct r; repeat constructor.
+  Qed.
+
+  Lemma read_hist_wf_bump (hist: read_hist) rop h rp
+    (RH_WF: read_hist_wf hist rop h)
+    (n := set_fold max 0 (dom hist)):
+  read_hist_auth hist
+    -∗ ith_rp n rp
+    ==∗
+  ∃ r rp',
+         let hist' := <[ n := ((r, h + 1), rp') ]> hist in
+         read_hist_auth hist' ∗ ith_read n r (h + 1) ∗ ⌜ read_hist_wf hist' rop (h + 1) ⌝ ∗
+         ith_rp n (upd_rp rp) ∗
+         ⌜ r <= h ⌝.
+  Proof using.
+    rewrite /read_hist_wf. iIntros "AUTH RP".
+    destruct RH_WF as (n_ & DOM & ROP & SEQ & BB).
+
+    assert (n_ = n) as ->.
+    { subst n. rewrite DOM. by rewrite dom_max_set_fold. }
+
+    destruct (hist !! n) as [[[r b0] p]| ] eqn:NTH.
+    2: { apply not_elem_of_dom in NTH. rewrite DOM in NTH.
+         rewrite elem_of_set_seq in NTH. lia. }
+    iDestruct (ith_rp_hist_compat with "[$] [$]") as %(? & ? & EQ').
+    rewrite NTH in H. inversion H. subst x. simpl in EQ'. clear H.
+    rename rp into p_. 
+    
+    iMod (read_hist_update' _ _ _ _ _ (h + 1) with "AUTH RP") as "(AUTH & #ITH & RP)".
+    { apply upd_rp_rs_step. }
+    { apply NTH. }
+
+    rewrite Nat.max_r.
+    2: { apply BB in NTH. simpl in NTH. lia. }
+    iModIntro. do 2 iExists _. iFrame "AUTH ITH RP".
+    iPureIntro. split.
+    2: { eapply BB in NTH; eauto. by apply NTH. }
+
+    exists n. split; [| split; [| split]]. 
+    - rewrite dom_insert_L. apply mk_is_Some, elem_of_dom in NTH. set_solver.
+    - done.
+    - intros ?????. rewrite !lookup_insert_Some.
+      intros [(? & ?) | (? & ITH) ] [(? & ?) | (? & JTH) ]; subst; simpl in *; try lia.
+      + apply mk_is_Some, elem_of_dom in JTH.
+        rewrite DOM elem_of_union elem_of_set_seq elem_of_singleton in JTH. lia.
+      + eapply SEQ in H; eauto. done.
+      + eapply SEQ; eauto.
+    - intros ??. rewrite lookup_insert_Some.         
+      intros [(? & ?) | (? & ITH) ]; subst; simpl; try lia.
+      { eapply BB in NTH; eauto. simpl in NTH. lia. }
+      eapply BB in ITH; eauto. lia.
+  Qed.
+
+  Lemma upd_rp_fin_pres rs
+    (FIN: rs_fin rs):
+    rs_fin (upd_rp rs).
+  Proof using.
+    red. destruct FIN; subst; simpl; try by eauto.
+    destruct H; subst; try by eauto.
+  Qed.
+
+  Lemma dequeue_upd_head_spec l τ π q h ph vh (nxh: loc) fl:
+    {{{ queue_inv l ∗
+        ith_node h (ph, (vh, nxh)) ∗ 
+        th_phase_frag τ π q ∗ cp_mul π d get_loc_fuel ∗
+        dequeue_resources h fl ph None }}}
+      #(Head q_sq) <- #nxh @τ
+    {{{ RET #(); th_phase_frag τ π q ∗ dequeue_resources (h + 1) fl nxh (Some h) ∗
+                   ∃ i r b, ith_read i r (h + 1) ∗ ⌜ r <= h ⌝ ∗
+                               br_lb b ∗
+                               (⌜ b < r ⌝ -∗ (ith_rp i rs_canceled ∨ ith_rp i (rs_proc (Some rsp_completed)))) }}}.
+  Proof using.
+    simpl.
+    iIntros (Φ) "([#QAT #INV] & #HTH & PH & CPS & DR) POST".
+    iInv "INV" as "(%hq & %h_ & %t & %br & %fl_ & %rop & %od_ & %hist & %ohv & inv)" "CLOS".
+    iEval (rewrite /queue_inv_inner) in "inv".
+    iDestruct "inv" as "(>HQ & >QI & >DANGLE & OHV & >%ORDER & >AUTHS & >ROP & >RHIST & >%RH_WF & >#OLDS & >RH & >DQ)".
+    iDestruct "DQ" as "[(% & DR') | TOK]".
+    { by iDestruct (dequeue_resources_excl with "[$] [$]") as "?". }
+    iDestruct (dequeue_resources_auth_agree with "[$] [$]") as %[<- <-]. 
+    iDestruct (dequeue_resources_dangle_agree with "[$] [$]") as %->.
+
+    iClear "INV QAT".
+
+    (* TODO: split into lemmas *)
+    iDestruct (hq_auth_lookup with "[$] [$]") as %HTH.
+    iAssert (⌜ t ≠ h ⌝)%I as %NEMPTY.
+    { iIntros (->). iDestruct (queue_interp_cur_empty with "[$]") as %NO.
+      specialize (NO 0). rewrite Nat.add_0_r in NO. congruence. }
+
+    rewrite /dangle_interp. iDestruct "DANGLE" as "(DAUTH & [_ | (% & ?)])"; [| done].
+    rewrite /dequeue_resources. iDestruct "DR" as "(CH & CFL & HEAD' & DFRAG)".
+    rewrite /queue_interp. iDestruct "QI" as "(%T_LEN &  HNIS & %pt & TAIL & TLI & %LL & HEAD & BR & FL)".
+    rewrite HTH. iEval (simpl) in "HEAD".
+
+    iCombine "HEAD HEAD'" as "HEAD". 
+    iApply sswp_MU_wp; [done| ].
+    iApply (wp_store with "[$]"). iIntros "!> [HEAD HEAD']".
+    MU_by_burn_cp. iApply wp_value.
+
+    iMod (dangle_update _ _ (Some h) with "[$] [$]") as "[DAUTH DFRAG]".
+
+    iAssert (|==> auths (h + 1) t br fl ∗ @me_exact _ q_me_h (h + 1))%I with "[CH AUTHS]" as "UPD".
+    { rewrite /auths. iDestruct "AUTHS" as "(AUTH&?&?&?)". iFrame.
+      iApply (me_update with "AUTH CH"). lia. }
+    iMod "UPD" as "[AUTHS CH]".
+
+    iApply "POST". iFrame.
+
+    iAssert (queue_interp hq (h + 1) t br fl ∗ hn_interp (ph, (vh, nxh)))%I
+      with "[HNIS TAIL TLI HEAD BR FL]" as "[QI HNI]".
+    { iFrame. rewrite -!bi.sep_assoc.
+      iSplit; [done| ].
+      iFrame "%".
+      pose proof (take_drop_middle _ _ _ HTH) as SPLIT.
+      rewrite -SPLIT.
+      assert (length (take h hq) = h) as H_LEN. 
+      { apply length_take_le. apply lookup_lt_Some in HTH. lia. }
+      rewrite drop_app_length'; [| done]. simpl.
+      rewrite cons_middle app_assoc.
+      rewrite drop_app_length'.
+      2: { rewrite length_app /=. lia. }
+      iDestruct "HNIS" as "[$ $]".
+      rewrite lookup_app_r.
+      2: { rewrite length_app /=. rewrite H_LEN. lia. }
+      rewrite length_app /=. rewrite H_LEN Nat.sub_diag. 
+      rewrite -SPLIT in LL. 
+      apply is_LL_into_drop with (k := h) in LL.
+      rewrite drop_app_length' in LL; [| done].
+      simpl in LL. destruct (drop (S h) hq) eqn:REST.
+      - by subst.
+      - simpl. destruct h0 as [? [??]]. simpl.
+        by destruct LL as [-> ?]. }
+
+    iDestruct (cancel_rop with "[$]") as "#CNC".
+    { red. rewrite Nat.add_1_r. reflexivity. }
+    
+    iDestruct (take_snapshot with "[$]") as "#SHT".
+    iDestruct "SHT" as "(_&_&#BR_LB&_)". 
+
+    rewrite /rop_interp.
+    destruct rop as [n| ]. 
+    - iDestruct ("ROP" with "[//]") as "(%r & %rp & READ_ & RP & ROP)".      
+      destruct RH_WF as (n' & DOM & [? | [=]] & RH_WF); [done| ]. subst n'. 
+      iMod (read_hist_wf_bump with "[$] [RP]") as "(%r' & %rp' & RHIST & #READ & %RH_WF' & RP & %READ_BOUND)".
+      { eexists. eauto. }
+      { rewrite DOM dom_max_set_fold. iFrame. }
+      rewrite DOM dom_max_set_fold. 
+      iDestruct (ith_read_agree with "READ READ_") as %<-.
+      iFrame "READ". iFrame "%". iFrame "BR_LB". 
+      rewrite -(bi.sep_True' ( ⌜ _ ⌝ -∗ _ )%I). iApply fupd_frame_l. iSplit.
+      { iIntros (LT). iDestruct "ROP" as "[SAFE | [-> _]]".
+        2: { iFrame. }
+        iDestruct "SAFE" as "[FROM_HEAD | [FROM_DANGLE | FROM_BR]]".
+        - iDestruct "FROM_HEAD" as "[-> [-> | (-> & -> & ?)]]".
+          + simpl. iFrame. 
+          + lia. 
+        - iDestruct "FROM_DANGLE" as "[(-> & -> & %X) ?]".
+          clear -X. by destruct X. 
+        - iDestruct "FROM_BR" as "([-> ->] & ->)". lia. } 
+
+      iClear "HTH CPS".
+      iMod ("CLOS" with "[-]") as "_"; [| done].
+      iFrame "QI AUTHS OHV HQ RH DAUTH TOK RHIST". iNext.
+      iExists _. rewrite Nat.add_sub. rewrite HTH /=.
+      
+      iSplitL "HNI". 
+      { iRight. by iFrame. }
+      iSplit.
+      { iPureIntro. red. red in ORDER. repeat split; try lia. }
+      rewrite DOM dom_max_set_fold in RH_WF'.
+      iFrame "%". 
+      iSplit.
+      2: { iApply old_rps_olds.
+           iDestruct (old_rps_olds with "OLDS") as "foo". 
+           by rewrite delete_insert_delete. }
+      rewrite /rop_interp. iIntros (i_ [=]). subst i_. 
+
+      iFrame "READ_ RP". 
+      iDestruct "ROP" as "[[HEAD | [DANGLE | FL]] | CANCEL_WITNESS]".
+      + iDestruct "HEAD" as "(-> & [-> | (-> & -> & TOK)])".
+        * iRight. simpl. by iFrame "#∗".
+        * iLeft. iRight. iLeft. iFrame.
+          iPureIntro. split.
+          ** split; [lia | done].
+          ** simpl. done. 
+      + iDestruct "DANGLE" as "((_ & _ & %) & _)". by destruct H.
+      + iDestruct "FL"as "([-> ->] & ->)". 
+        iLeft. rewrite /safe_read.
+        repeat iRight. done.
+      + iDestruct "CANCEL_WITNESS" as "(-> & CW)".
+        iRight. by iFrame.
+    - destruct RH_WF as (n & DOM & [? | [=]] & RH_WF).
+      destruct (hist !! n) as [[[??]?] | ] eqn:NTH. 
+      2: { apply not_elem_of_dom in NTH. rewrite DOM in NTH.
+           rewrite elem_of_set_seq in NTH. lia. }
+      iDestruct (big_sepM_lookup  with "OLDS") as "RP".
+      { simpl. apply NTH. } 
+      iDestruct "RP" as "(%rp & RP & %FIN & #LB)".
+      iDestruct (ith_rp_hist_compat with "[$] [$]") as %(? & ? & LE').
+      rewrite NTH in H0. inversion H0. subst x. simpl in *.
+
+      iDestruct (read_hist_get hist n with "RHIST") as "#READ".
+      { rewrite NTH. repeat f_equal. }
+      
+      iMod (read_hist_wf_bump with "[$] [RP]") as "(%r' & %rp' & RHIST & #READ' & %RH_WF' & RP_ & %READ_BOUND)".
+      { eexists. eauto. }
+      { rewrite DOM dom_max_set_fold. iFrame "RP". }
+      rewrite DOM dom_max_set_fold.
+      iDestruct (ith_read_agree with "READ READ'") as %->.
+      iFrame "% READ' BR_LB".
+      rewrite -(bi.sep_True' ( ⌜ _ ⌝ -∗ _ )%I). iApply fupd_frame_l. iSplit.
+      { iIntros (LT). destruct FIN as [-> | [-> | ->]].
+        all: try by iFrame.
+        iDestruct (br_lb_bound with "[$] [$]") as %?. lia. }
+
+      iMod ("CLOS" with "[-]") as "_"; [| done].
+      iFrame "QI AUTHS OHV HQ RH DAUTH TOK RHIST". iNext.
+      iExists _. rewrite Nat.add_sub. rewrite HTH /=.
+      
+      iSplitL "HNI". 
+      { iRight. by iFrame. }
+      iSplit.
+      { iPureIntro. red. red in ORDER. repeat split; try lia. }
+      rewrite DOM dom_max_set_fold in RH_WF'.
+      (* do 2 (rewrite decide_False in RH_WF'; [| destruct FIN as [->| [->| ->]]; done]). *)
+      destruct RH_WF as (SEQ &  BB). 
+      Unshelve. 2: exact None. 
+      rewrite bi.sep_assoc.      
+      iSplitR.
+      2: { (* TODO: make a lemma? *)
+        rewrite /old_rps. simpl.
+        rewrite -insert_delete_insert.         
+        rewrite insert_union_singleton_l big_sepM_union.
+        2: { apply map_disjoint_dom. rewrite dom_insert_L. set_solver. }
+        iSplitL.
+        2: { iApply (big_sepM_subseteq with "[$]"). apply delete_subseteq. }
+        rewrite big_sepM_singleton. iFrame. iFrame "% #".
+        iPureIntro. by apply upd_rp_fin_pres. }
+      rewrite /rop_interp. iSplit. 
+      { iIntros (i_ [=]). }
+
+      (* TODO: make a lemma *)
+      rewrite /read_hist_wf.
+      iPureIntro. 
+
+      exists n. split; [| split; [| split]]. 
+    + rewrite dom_insert_L. apply mk_is_Some, elem_of_dom in NTH. set_solver.
+    + tauto. 
+    + intros ?????. rewrite !lookup_insert_Some.
+      intros [(? & ?) | (? & ITH) ] [(? & ?) | (? & JTH) ]; subst; simpl in *; try lia.
+      * apply mk_is_Some, elem_of_dom in JTH.
+        rewrite DOM elem_of_union elem_of_set_seq elem_of_singleton in JTH. lia.
+      * eapply SEQ in H1; eauto. done.
+      * eapply SEQ; eauto.
+    + intros ??. rewrite lookup_insert_Some.         
+      intros [(? & ?) | (? & ITH) ]; subst; simpl; try lia.
+      eapply BB in ITH; eauto. simpl in ITH. lia.
+  Qed.
+
+  Definition dequeue_fuel := 100.    
+
+  Lemma check_BR_spec l τ π q h fl ph ndh i r b0
+    (READ_BOUND: r <= h):
+    {{{ queue_inv l ∗
+        ith_node h (ph, ndh) ∗
+        dequeue_resources (h + 1) fl ndh.2 (Some h) ∗ 
+        th_phase_frag τ π q ∗ cp_mul π d get_loc_fuel ∗
+        ith_read i r (h + 1) ∗ br_lb b0
+    }}}
+      ! #(BeingRead q_sq) @τ
+    {{{ (pbr: loc), RET #pbr; th_phase_frag τ π q ∗
+            dequeue_resources (h + 1) fl ndh.2 (if (decide (pbr = ph)) then Some h else None) ∗
+            (⌜ pbr = ph ⌝ ∨ 
+             ⌜ pbr ≠ ph ⌝ ∗ hn_interp (ph, ndh)) ∗
+            ∃ b' ndbr', br_lb b' ∗ ⌜ b0 <= b' ⌝ ∗ ith_node b' (pbr, ndbr')
+    }}}.
+  Proof using.
+    iIntros (Φ) "([#QAT #INV] & #HTH & DR& PH & CPS & #READ & #BR0) POST".
+    iInv "INV" as "(%hq & %h_ & %t & %br & %fl_ & %rop & %od_ & %hist & %ohv & inv)" "CLOS".
+    iEval (rewrite /queue_inv_inner) in "inv".
+    iDestruct "inv" as "(>HQ & >QI & >DANGLE & OHV & >%ORDER & >AUTHS & >ROP & >RHIST & >%RH_WF & >#OLDS & >RH & >DQ)".
+    iDestruct "DQ" as "[(% & DR') | TOK]".
+    { by iDestruct (dequeue_resources_excl with "[$] [$]") as "?". }
+    iDestruct (dequeue_resources_auth_agree with "[$] [$]") as %[<- <-]. 
+    iDestruct (dequeue_resources_dangle_agree with "[$] [$]") as %->.
+
+    iClear "INV QAT".
+
+    (* TODO: split into lemmas *)
+    iDestruct (hq_auth_lookup with "[$] [$]") as %HTH.
+    iAssert (⌜ t ≠ h ⌝)%I as %NEMPTY.
+    { iIntros (->). red in ORDER. lia. }
+
+    rewrite /dangle_interp. iDestruct "DANGLE" as "(DAUTH & [% | (_ & HNI)])"; [done| ].
+    rewrite Nat.add_sub HTH /=. 
+    rewrite /dequeue_resources. iDestruct "DR" as "(CH & CFL & HEAD' & DFRAG)".
+    rewrite /queue_interp. iDestruct "QI" as "(%T_LEN &  HNIS & %pt & TAIL & TLI & %LL & HEAD & BR & FL)".
+    iDestruct "BR" as "(%nbr & %BRTH & BR)". destruct nbr as [pbr nbr].
+
+    iApply sswp_MU_wp; [done| ]. 
+    iApply (wp_load with "BR"). iIntros "!> BR".
+    MU_by_burn_cp. iApply wp_value.
+
+    iApply "POST". iFrame.
+
+    iDestruct (br_lb_bound with "BR0 AUTHS") as %BR0. 
+    iDestruct (take_snapshot with "[$]") as "#SHT".
+    iDestruct (hq_auth_get_ith with "HQ") as "#BRTH'".
+    { apply BRTH. }
+    iFrame "BRTH'". 
+
+    iAssert (queue_interp hq (h + 1) t br fl)%I
+      with "[HNIS TAIL TLI HEAD BR FL]" as "QI".
+    { by iFrame. }
+    iAssert (br_lb br ∗ ⌜b0 ≤ br⌝)%I as "$".
+    { iSplit; [| done].
+      iDestruct "SHT" as "(?&?&?&?)". done. }
+
+    simpl.
+    destruct (decide (pbr = ph)) as [-> | NEQ].
+    -
+      iFrame. 
+      iMod ("CLOS" with "[-]") as "_".
+      { iFrame "#∗ %". iNext.
+        rewrite Nat.add_sub HTH /=.
+        iRight. by iFrame. }
+      iModIntro. by iLeft.
+    - iDestruct (ith_read_hist_compat with "[$] [$]") as %(b & p & READ & INCR_BOUND). 
+      iMod (dangle_update _ _ None with "[$] [$]") as "[DAUTH DFRAG]".
+      iFrame.      
+      iApply fupd_or. iRight. iFrame "HNI".
+      rewrite -(bi.sep_True' ⌜ _ ≠ _ ⌝%I). iApply fupd_frame_l. iSplit; [done| ].
+      iMod ("CLOS" with "[-]") as "_"; [| done]. 
+
+      rewrite /rop_interp.
+      destruct rop.
+      2: { iFrame "#∗ %". iNext. iSplitR.
+           { by iLeft. }
+           rewrite /rop_interp. by iIntros (??). }
+      
+      iDestruct ("ROP" with "[//]") as "(%r_ & %rp & READ_ & RP & ROP)".
+      iDestruct (ith_read_hist_compat with "[$] READ_") as %(?&? & READ' & _). 
+
+      iFrame. iFrame "OLDS".
+      iNext. iSplitR.
+      { by iLeft. }
+      iSplit; [done| ]. iSplit; [| done]. 
+      rewrite /rop_interp.
+      iIntros (i' [=]). subst n.
+      iDestruct "ROP" as "[SAFE | $]".
+      2: { iFrame "#∗". }
+
+      destruct (decide (i' = i)). 
+      { subst. rewrite {1}/safe_read. rewrite Nat.add_sub.
+        iFrame "READ_". 
+        iDestruct "SAFE" as "[FROM_HEAD | [FROM_DANGLE | FROM_BR]]".
+        - iFrame.
+        - iDestruct "FROM_DANGLE" as "[(-> & -> & _) ?]".
+          congruence.
+        - iFrame. }
+
+      assert (i < i') as NEW.
+      { red in RH_WF. destruct RH_WF as (n' & DOM & [? | [=]] & RH_WF); [done| ].
+        subst i'.
+        apply mk_is_Some, elem_of_dom in READ. rewrite DOM elem_of_set_seq in READ.
+        lia. }
+      clear n.
+      
+      assert (h + 1 <= r_) as READ'_BOUND.
+      { red in RH_WF. destruct RH_WF as (n' & DOM & [? | [=]] & RH_WF); [done| ].
+        subst. 
+        apply proj1 in RH_WF. eapply RH_WF in NEW; eauto. simpl in NEW. lia. }
+      iFrame "READ_".
+      rewrite {1}/safe_read.
+      iDestruct "SAFE" as "[FROM_HEAD | [FROM_DANGLE | FROM_BR]]".
+      + iFrame.
+      + iDestruct "FROM_DANGLE" as "[(-> & -> & _) ?]". lia.
+      + iFrame.
+  Qed.
+
+  Lemma read_FL_spec τ π l h q fl nd od:
+  {{{ queue_inv l ∗ dequeue_resources h fl nd od ∗
+      cp π d ∗ th_phase_frag τ π q }}}
+    ! #(FreeLater q_sq) @τ
+  {{{ (pfl: loc), RET (#pfl);
+      ∃ ndfl, ith_node fl (pfl, ndfl) ∗ 
+      dequeue_resources h fl nd od ∗ th_phase_frag τ π q }}}.
+  Proof using.
+    iIntros (Φ) "([#QAT #INV] & DR & CPS & PH) POST".
+    iInv "INV" as "(%hq & %h_ & %t & %br & %fl_ & %rop & %od_ & %hist & %ohv & inv)" "CLOS".
+    iEval (rewrite /queue_inv_inner) in "inv".
+    iDestruct "inv" as "(>HQ & >QI & >DANGLE & OHV & >%ORDER & >AUTHS & >ROP & >RHIST & >%RH_WF & >#OLDS & >RH & >DQ)".
+    iDestruct "DQ" as "[(% & DR') | TOK]".
+    { by iDestruct (dequeue_resources_excl with "[$] [$]") as "?". }
+    iDestruct (dequeue_resources_auth_agree with "[$] [$]") as %[<- <-].
+    rewrite /queue_interp. iDestruct "QI" as "(%T_LEN &  HNIS & %pt & TAIL & TLI & %LL & HEAD & BR & FL)".
+    iDestruct "FL" as "(%x & %FLTH & FL & HNI_FL)". 
+    iDestruct (hq_auth_get_ith with "[$]") as "#FLTH"; [by eauto| ].
+    iApply sswp_MU_wp; [done| ].     
+    iApply (wp_load with "FL"). iIntros "!> FL".
+    rewrite cp_mul_1. 
+    MU_by_burn_cp. iApply wp_value.
+    iMod ("CLOS" with "[-POST DR PH]") as "_".
+    { iFrame. iFrame "OLDS". done. }
+    iModIntro. iApply "POST". iFrame.
+    destruct x. iFrame "FLTH".     
+  Qed.
+
+  Lemma get_to_free_spec 
+    l τ π q h fl (ph: loc) ndh i r b
+    (READ_BOUND: r <= h):
+    {{{ queue_inv l ∗
+        ith_node h (ph, ndh) ∗
+        dequeue_resources (h + 1) fl ndh.2 (Some h) ∗ 
+        th_phase_frag τ π q ∗ cp_mul π d (get_loc_fuel + get_loc_fuel + get_loc_fuel) ∗
+        ith_read i r (h + 1) ∗
+        br_lb b ∗ (⌜ b < r ⌝ -∗ (ith_rp i rs_canceled ∨ ith_rp i (rs_proc (Some rsp_completed))))
+    }}}
+      get_to_free q_sq #ph @ τ
+    {{{ (to_free: loc), RET #to_free;
+        ∃ hn fl', hn_interp (to_free, hn) ∗ th_phase_frag τ π q ∗
+                    dequeue_resources (h + 1) fl' ndh.2 None }}}.
+  Proof using.
+    simpl.
+    iIntros (Φ) "([#QAT #INV] & #HTH & DR& PH & CPS & #READ & #BR0 & #NO_FL) POST".
+    rewrite /get_to_free. destruct q_sq eqn:Q_SQ. 
+    pure_steps. 
+    
+    split_cps "CPS" get_loc_fuel.
+    wp_bind (! _)%E. 
+    replace BeingRead0 with (BeingRead q_sq) by (by rewrite Q_SQ). 
+    iApply (check_BR_spec with "[-POST CPS]").
+    { apply READ_BOUND. }
+    { iFrame "#∗". }
+    iIntros "!> %pbr (PH & DR & RES)".
+    iDestruct "RES" as "(RES & %b1 & %ndbr1 & #BR1 & %LEb & #BRTH1)". 
+
+    wp_bind (_ = _)%E.
+    iApply sswp_MU_wp; [done| ].
+    iApply sswp_pure_step.
+    { set_solver. }
+    MU_by_burn_cp. iApply wp_value.
+
+    iDestruct "RES" as "[%PTR_EQ | [%NEQ HNI]]".
+    2: { rewrite bool_decide_false; [| set_solver]. rewrite decide_False; [| done].
+         pure_steps. iApply "POST". iFrame. }
+
+    rewrite PTR_EQ. 
+
+    rewrite bool_decide_true; [| set_solver]. rewrite decide_True; [| done].
+    pure_steps.
+
+    wp_bind (! _)%E.
+    split_cps "CPS" 1. rewrite -cp_mul_1.
+    replace FreeLater0 with (FreeLater q_sq) by (by rewrite Q_SQ). 
+    iApply (read_FL_spec with "[-POST CPS]").
+    { iFrame "#∗". }
+    iIntros "!> %pfl (%ndfl & #FLTH & DR & PH)".
+
+    wp_bind (Rec _ _ _)%E. pure_steps.
+
+    wp_bind (_ <- _)%E.
+
+    iInv "INV" as "(%hq & %h_ & %t & %br & %fl_ & %rop & %od_ & %hist & %ohv & inv)" "CLOS".
+    iEval (rewrite /queue_inv_inner) in "inv".
+    iDestruct "inv" as "(>HQ & >QI & >DANGLE & OHV & >%ORDER & >AUTHS & >ROP & >RHIST & >%RH_WF & >#OLDS & >RH & >DQ)".
+    iDestruct "DQ" as "[(% & DR') | TOK]".
+    { by iDestruct (dequeue_resources_excl with "[$] [$]") as "?". }
+    iDestruct (dequeue_resources_auth_agree with "[$] [$]") as %[<- <-]. 
+    iDestruct (dequeue_resources_dangle_agree with "[$] [$]") as %->.
+
+    iClear "INV QAT".
+
+    (* TODO: split into lemmas *)
+    iDestruct (hq_auth_lookup with "[$] HTH") as %HTH.
+    iAssert (⌜ t ≠ h ⌝)%I as %NEMPTY.
+    { iIntros (->). red in ORDER. lia. }
+
+    iPoseProof (queue_interp_dangle_neq_pfl' _ _ _ _ _ ph with "QI [DANGLE]") as "#PFL_NEQ_D".
+    { by rewrite Nat.add_sub. }
+
+    rewrite /dangle_interp. iDestruct "DANGLE" as "(DAUTH & [% | (_ & HNI)])"; [done| ].
+    rewrite Nat.add_sub HTH /=. 
+    rewrite /dequeue_resources. iDestruct "DR" as "(CH & CFL & HEAD' & DFRAG)".
+
+    
+    rewrite /queue_interp. iDestruct "QI" as "(%T_LEN &  HNIS & %pt & TAIL & TLI & %LL & HEAD & BR & FL)".
+    iDestruct "BR" as "(%nbr & %BRTH & BR)".
+    
+    iDestruct (br_lb_bound with "BR1 AUTHS") as %BR1. 
+
+    subst pbr. 
+    destruct nbr as [pbr nbr].
+
+    (* iCombine "HEAD HEAD'" as "HEAD".  *)
+    iApply sswp_MU_wp; [done| ].
+
+    iDestruct "FL" as "(%ndfl_ & %FLTH & FL & HNI_FL)".
+    iDestruct (hq_auth_lookup with "[$] FLTH") as %FLTH_.
+    rewrite FLTH in FLTH_. inversion FLTH_. subst ndfl_. clear FLTH_. 
+    iApply (wp_store with "FL"). iIntros "!> FL".
+    MU_by_burn_cp. iApply wp_value.
+
+    iMod (dangle_update _ _ None with "[$] [$]") as "[DAUTH DFRAG]".
+    iAssert (|==> auths (h + 1) t br h ∗ @me_exact _ q_me_fl h)%I with "[CFL AUTHS]" as "UPD".
+    { rewrite /auths. iDestruct "AUTHS" as "(?&?&?&A)". iFrame.
+      iApply (me_update with "A CFL"). red in ORDER. lia. }
+    iMod "UPD" as "[AUTHS CFL]".
+
+    iDestruct (br_lb_bound with "BR0 [$]") as %BR0. 
+    iAssert (queue_interp hq (h + 1) t br h)%I
+      with "[HNIS TAIL TLI HEAD BR FL HNI]" as "QI".
+    { iFrame. 
+      iSplit; [done| ].
+      iFrame "%". iFrame. } 
+
+    rewrite /rop_interp.
+    destruct rop. 
+    - iDestruct ("ROP" with "[//]") as "(%r_ & %rp & READ_ & RP & ROP)".
+      iDestruct (ith_read_hist_compat with "[$] READ_") as %(?&? & READ' & _). 
+      iDestruct (ith_read_hist_compat with "[$] READ") as %(?&? & READ & BB).
+      iDestruct (hq_auth_lookup with "[$] BRTH1") as %BRTH1.
+      
+      iAssert (dequeue_resources (h + 1) h ndh.2 None)%I with "[CH CFL HEAD' DFRAG]" as "DR".
+      { iFrame. }
+
+      iMod ("CLOS" with "[-POST CPS PH DR HNI_FL]") as "_".
+      { iFrame. iExists _. iNext. iSplitR.
+        { by iLeft. }        
+        iFrame "%". iFrame "OLDS". 
+        iSplit; cycle 1.
+        - rewrite /rop_interp.
+          iIntros (i' [=]). subst n.
+          iDestruct "ROP" as "[SAFE | $]".
+          2: { iFrame. }
+          iFrame "READ_".
+          
+          destruct (decide (i' = i)). 
+          { subst. rewrite {1}/safe_read. rewrite Nat.add_sub.
+            iDestruct "SAFE" as "[FROM_HEAD | [FROM_DANGLE | FROM_BR]]".
+            - iFrame.
+            - iDestruct "FROM_DANGLE" as "[(-> & -> & _) ->]".
+              iFrame "RP". 
+              iLeft. rewrite /safe_read. rewrite Nat.add_sub.
+              do 2 iRight. by iFrame. 
+            - iDestruct "FROM_BR" as "([-> ->] & ->)". 
+              rewrite READ in READ'. inversion READ'. subst r x1 x2.
+              apply Nat.le_lteq in BR0 as [BR0 | ->].
+              { iSpecialize ("NO_FL" with "[//]"). iExFalso.
+                iAssert (∃ rp', ith_rp i rp' ∗ ⌜ rp' = rs_canceled \/ rp' = (rs_proc (Some rsp_completed))⌝)%I as "(%rp' & RP' & %RP')".
+                { iDestruct "NO_FL" as "[$|$]"; set_solver. }
+                iDestruct (ith_rp_le with "RP RP'") as %CM.
+                exfalso. clear -RP' CM.
+                inversion CM; destruct RP' as [-> | ->]; try done.
+                subst. inversion RSP. by subst. }
+              rename x into bi.
+              red in RH_WF.
+              destruct RH_WF as (n' & DOM & [? | [=]] & SEQ & BB'); [done| ].
+              subst n'.
+              pose proof READ as EQ%BB'. simpl in EQ.
+              assert (bi = h + 1) as -> by lia.  clear BB EQ.
+              assert (b1 = fl) as -> by lia.
+              rewrite BRTH in BRTH1. inversion BRTH1. subst pbr ndbr1.
+              iDestruct ("PFL_NEQ_D" with "[] []") as "?".
+              { eauto. }
+              { eauto. }
+              done. }
+          
+          assert (i < i') as NEW.
+          { red in RH_WF. destruct RH_WF as (n' & DOM & [? | [=]] & RH_WF); [done| ].
+            subst i'.
+            apply mk_is_Some, elem_of_dom in READ. rewrite DOM elem_of_set_seq in READ.
+            lia. }
+          clear n.
+
+          assert (h + 1 <= r_) as READ'_BOUND.
+          { red in RH_WF. destruct RH_WF as (n' & DOM & [? | [=]] & RH_WF); [done| ].
+            apply proj1 in RH_WF. eapply RH_WF in NEW; eauto. simpl in NEW. lia. }
+          rewrite {1}/safe_read.
+          iDestruct "SAFE" as "[FROM_HEAD | [FROM_DANGLE | FROM_BR]]".
+          + iFrame.
+          + iDestruct "FROM_DANGLE" as "[(-> & -> & _) ?]". lia.
+          + iFrame.
+            iDestruct "FROM_BR" as "([% %] & ?)". subst.
+            red in ORDER. lia.
+        - rewrite /hq_state_wf. iPureIntro.
+          red in ORDER. lia. }
+
+      iModIntro. wp_bind (Rec _ _ _)%E. pure_steps.
+      iApply "POST". iFrame. 
+    - 
+      iAssert (dequeue_resources (h + 1) h ndh.2 None)%I with "[CH CFL HEAD' DFRAG]" as "DR".
+      { iFrame. }
+
+      iMod ("CLOS" with "[-POST CPS PH DR HNI_FL]") as "_".
+      { iFrame. iExists _. iNext. iSplitR.
+        { by iLeft. }
+        iFrame "% OLDS".
+        iSplit; cycle 1.
+        - rewrite /rop_interp. by iIntros (??). 
+        - rewrite /hq_state_wf. iPureIntro.
+          red in ORDER. lia. }
+
+      iModIntro. wp_bind (Rec _ _ _)%E. pure_steps.
+      iApply "POST". iFrame. 
+  Qed.
+
+  Lemma free_el_spec τ π q ptr nd:
+    {{{ th_phase_frag τ π q ∗ cp_mul π d get_loc_fuel ∗ 
+        hn_interp (ptr, nd) }}}
+      free_el #ptr @ τ
+    {{{ v, RET v; th_phase_frag τ π q }}}.
+  Proof using. Admitted. 
+  
+  Lemma dequeue_spec l (τ: locale heap_lang) (π: Phase) (q: Qp):
+    {{{ queue_inv l ∗ dequeue_token ∗ 
+        th_phase_frag τ π q ∗ cp_mul π d dequeue_fuel }}}
+      dequeue q_sq l @ τ
+    {{{ (v: val), RET v; th_phase_frag τ π q ∗ dequeue_token }}}.
+  Proof using.
+    simpl. iIntros (Φ) "([#QAT #INV] & TOK & PH & CPS) POST".
+    rewrite /dequeue. destruct q_sq eqn:Q_SQ.
+    pure_steps.
+
+    wp_bind (! _)%E.
+    iInv "INV" as "(%hq & %h & %t & %br & %fl & %rop & %od & %hist & %ohv & inv)" "CLOS".
+    iEval (rewrite /queue_inv_inner) in "inv".
+    iDestruct "inv" as "(>HQ & >QI & >DANGLE & OHV & >%ORDER & >AUTHS & >ROP & >RHIST & >%RH_WF & >#OLDS & >RH & >DQ)".
+    
+    iApply sswp_MU_wp; [done| ].
+    iDestruct (access_queue_ends with "[$] [$]") as "(%ph & %pt & HEAD & TAIL & HT & CLOS')".
+    replace Head0 with (Head q_sq) by (by rewrite Q_SQ).
+    iApply (wp_load with "HEAD"). iIntros "!> HEAD".
+    iDestruct "DQ" as "[[%ph_ DR] | TOK']".
+    2: { by iDestruct (dequeue_token_excl with "[$] [$]") as "?". }
+    iDestruct (dequeue_res_head_agree with "DR [$]") as %<-. 
+    iDestruct (dequeue_resources_dangle_agree with "DR [$]") as %->.
+    iDestruct ("CLOS'" with "[$] [$]") as "(HQ & QI)".
+    MU_by_burn_cp. iApply wp_value.
+
+    iMod ("CLOS" with "[-POST CPS PH DR]") as "_".
+    { iFrame. by iFrame "OLDS". }
+    iModIntro.
+
+    (* TODO: do we need to keep track of previous values at this point? *)
+    clear t br ohv ORDER hq.
+    iClear "OLDS". 
+    clear pt rop RH_WF hist.
+
+    wp_bind (Rec _ _ _)%E. pure_steps. 
+    
+    wp_bind (! _)%E.
+    iInv "INV" as "(%hq & %h_ & %t & %br & %fl_ & %rop & %od_ & %hist & %ohv & inv)" "CLOS".
+    iEval (rewrite /queue_inv_inner) in "inv".
+    iDestruct "inv" as "(>HQ & >QI & >DANGLE & OHV & >%ORDER & >AUTHS & >ROP & >RHIST & >%RH_WF & >#OLDS & >RH & >DQ)".
+    iApply sswp_MU_wp; [done| ].
+    iDestruct (access_queue_ends with "[$] [$]") as "(%ph_ & %pt & HEAD & TAIL & #HT & CLOS')".
+    replace Tail0 with (Tail q_sq) by (by rewrite Q_SQ).
+    iApply (wp_load with "[$]"). iIntros "!> TAIL".
+    iDestruct (dequeue_res_head_agree with "DR [$]") as %->. 
+    iDestruct (dequeue_resources_auth_agree with "DR [$]") as %[<- <-].
+    iDestruct (take_snapshot with "[$]") as "#SHT".
+    iDestruct "DQ" as "[(% & DR') | TOK]".
+    { by iDestruct (dequeue_resources_excl with "DR DR'") as "?". }
+
+    iDestruct ("CLOS'" with "[$] [$]") as "(HQ & QI)".
+    MU_by_burn_cp. iApply wp_value.
+    iMod ("CLOS" with "[-POST CPS PH DR]") as "_".
+    { iFrame. by iFrame "OLDS". }
+    iModIntro.
+
+    (* TODO: do we need to keep track of previous values at this point? *)
+    (* clear br hob od ohv ORDER SAFE_BR hq. *)
+    iClear "OLDS SHT". 
+    clear ohv hist hq RH_WF od_ (* ORDER *) rop (* br *).    
+
+    wp_bind (_ = _)%E.
+    iApply sswp_MU_wp; [done| ].
+    iApply sswp_pure_step.
+    { set_solver. }
+    MU_by_burn_cp. iApply wp_value.
+
+    (* destruct bool_decide. *)
+    iDestruct "HT" as "[[%GE <-] | (%NEMPTY & %ndh & #HTH)]". 
+    { assert (t = h) as ->.
+      { red in ORDER. lia. }
+      rewrite bool_decide_true; [| done]. 
+      iApply sswp_MU_wp_fupd; [done| ]. 
+      iInv "INV" as "(%hq & %h_ & %t & %br' & %fl_ & %rop & %od_ & %hist & %ohv & inv)" "CLOS".
+      iEval (rewrite /queue_inv_inner) in "inv".
+      iDestruct "inv" as "(>HQ & >QI & >DANGLE & OHV & >%ORDER' & >AUTHS & >ROP & >RHIST & >%RH_WF & >#OLDS & >RH & >DQ)".
+      iModIntro.
+      iApply sswp_pure_step; [done| ].
+      do 2 iNext. MU_by_burn_cp.
+      iDestruct "DQ" as "[(% & DR') | TOK]".
+      { by iDestruct (dequeue_resources_excl with "[$] [$]") as "?". }
+      iDestruct (dequeue_resources_auth_agree with "[$] [$]") as %[-> ->]. 
+      iMod ("CLOS" with "[-POST CPS PH TOK]") as "_".
+      { iFrame. by iFrame "OLDS". }
+      iModIntro. pure_steps.
+      iApply "POST". iFrame. }
+
+    rewrite bool_decide_false; [| set_solver]. pure_steps.
+    split_cps "CPS" get_loc_fuel; [cbv; lia| ].  
+    iApply (get_head_val_spec with "[-POST CPS]").
+    { iFrame "#∗". }
+    iIntros "!> [PH DR]".
+    wp_bind (Rec _ _ _)%E. pure_steps.
+
+    destruct ndh as [vh nxh]. simpl.
+    wp_bind (_ <- _)%E.
+    replace OldHeadVal0 with (OldHeadVal q_sq) by (by rewrite Q_SQ).
+    split_cps "CPS" get_loc_fuel; [cbv; lia| ].     
+    iApply (update_ohv_spec with "[$QAT $PH $CPS' $INV]").
+    iIntros "!> PH".
+    wp_bind (Rec _ _ _)%E. pure_steps.
+
+    split_cps "CPS" get_loc_fuel; [cbv; lia| ].
+    iApply (get_head_next_spec with "[-POST CPS]").
+    { iFrame "#∗". }
+    iIntros "!> [PH DR]". simpl.
+
+    wp_bind (_ <- _)%E.
+    split_cps "CPS" get_loc_fuel; [cbv; lia| ].
+    iApply (dequeue_upd_head_spec with "[$QAT $CPS' $PH $INV $HTH $DR]").
+    iIntros "!> (PH & DR & (%i & %r & %b & #ITHR & %BR & #TOKS))".
+
+    wp_bind (Rec _ _ _)%E. do 3 pure_step_cases.
+    fold (get_to_free (SQ Head0 Tail0 BeingRead0 FreeLater0 OldHeadVal0)).
+    rewrite -Q_SQ. 
+    wp_bind (get_to_free _ _)%E.         
+    split_cps "CPS" (3 * get_loc_fuel); [cbv; lia| ].
+    iApply (get_to_free_spec with "[-POST CPS]").
+    { apply BR. }
+    { iFrame "#∗". }
+    
+    iIntros "!> %to_free (%hfr & %fl' & HNFR & PH & DR)".
+    wp_bind (Rec _ _ _)%E. pure_steps.
+    wp_bind (free_el _)%E.
+    split_cps "CPS" get_loc_fuel; [cbv; lia| ].
+    iApply (free_el_spec with "[CPS' PH HNFR]").
+    { iFrame. }
+    iIntros "!> %v PH".
+
+    wp_bind (Rec _ _ _)%E. do 2 pure_step_cases. 
+    iClear "TOKS ITHR HTH". 
+    clear dependent r t hfr to_free br ph b. 
+
+    iApply sswp_MU_wp_fupd; [done| ]. 
+    iInv "INV" as "(%hq & %h_ & %t & %br & %fl_ & %rop & %od & %hist & %ohv & inv)" "CLOS".
+    iEval (rewrite /queue_inv_inner) in "inv".
+    iDestruct "inv" as "(>HQ & >QI & >DANGLE & OHV & >%ORDER & >AUTHS & >ROP & >RHIST & >%RH_WF & >#OLDS & >RH & >DQ)".
+    iDestruct "DQ" as "[(% & DR') | TOK]".
+    { by iDestruct (dequeue_resources_excl with "DR DR'") as "?". }
+    (* iDestruct (dequeue_res_head_agree with "DR [$]") as %->.  *)
+    iDestruct (dequeue_resources_auth_agree with "DR [$]") as %[<- <-].
+    iDestruct (dequeue_resources_dangle_agree with "DR [$]") as %->.
+
+    iModIntro. iApply sswp_pure_step; [done| ]. 
+    MU_by_burn_cp. simpl.
+    iMod ("CLOS" with "[-POST CPS PH TOK]") as "_".
+    { iFrame. by iFrame "OLDS". }
+ 
+    iModIntro. pure_steps.
+    iApply "POST". iFrame.
+  Qed.
+
+  Print Assumptions dequeue_spec.
+    
+End Dequeue.
